access: Arch_AC arch split
Signed-off-by: Ryan Barry <ryan.barry@unsw.edu.au>

proof/access-control/Arch_AC.thy
@@ -5,389 +5,37 @@
  *)
 
 theory Arch_AC
-imports Retype_AC
+imports ArchRetype_AC
 begin
-
-context begin interpretation Arch . (*FIXME: arch_split*)
 
 text\<open>
 
-Arch-specific access control.
+Setup for arch-specific access control.
 
 \<close>
 
-lemma store_pde_respects:
-  "\<lbrace>integrity aag X st and K (is_subject aag (p && ~~ mask pd_bits)) \<rbrace>
-     store_pde p pde
-   \<lbrace>\<lambda>rv. integrity aag X st\<rbrace>"
-  apply (simp add: store_pde_def set_pd_def)
-  apply (wp get_object_wp set_object_integrity_autarch)
-  apply simp
-  done
+(* c.f.  auth_ipc_buffers *)
+definition ipc_buffer_has_auth :: "'a PAS \<Rightarrow> obj_ref \<Rightarrow> obj_ref option \<Rightarrow> bool" where
+   "ipc_buffer_has_auth aag thread \<equiv>
+    case_option True (\<lambda>p. is_aligned p msg_align_bits \<and>
+                          (\<forall>x \<in> ptr_range p msg_align_bits. abs_has_auth_to aag Write thread x))"
 
-lemma store_pte_respects:
-  "\<lbrace>integrity aag X st and K (is_subject aag (p && ~~ mask pt_bits)) \<rbrace>
-     store_pte p pte
-   \<lbrace>\<lambda>rv. integrity aag X st\<rbrace>"
-  apply (simp add: store_pte_def set_pt_def)
-  apply (wp get_object_wp set_object_integrity_autarch)
-  apply simp
-  done
+lemma ipc_buffer_has_auth_wordE:
+  "\<lbrakk> ipc_buffer_has_auth aag thread (Some buf); p \<in> ptr_range (buf + off) sz;
+     is_aligned off sz; sz \<le> msg_align_bits; off < 2 ^ msg_align_bits \<rbrakk>
+     \<Longrightarrow> abs_has_auth_to aag Write thread p"
+  unfolding ipc_buffer_has_auth_def
+  by (fastforce elim: bspec set_mp[OF ptr_range_subset])
 
-lemma integrity_arch_state [iff]:
-  "\<lbrakk>arm_asid_table v = arm_asid_table (arch_state s)\<rbrakk> \<Longrightarrow>
-   integrity aag X st (s\<lparr>arch_state := v\<rparr>) = integrity aag X st s"
-  unfolding integrity_def
-  by (simp )
-
-lemma integrity_arm_asid_map [iff]:
-  "integrity aag X st (s\<lparr>arch_state := ((arch_state s)\<lparr>arm_asid_map := v\<rparr>)\<rparr>) = integrity aag X st s"
-  unfolding integrity_def
-  by (simp )
-
-lemma integrity_arm_hwasid_table [iff]:
-  "integrity aag X st (s\<lparr>arch_state := ((arch_state s)\<lparr>arm_hwasid_table := v\<rparr>)\<rparr>) = integrity aag X st s"
-  unfolding integrity_def
-  by (simp )
-
-lemma integrity_arm_next_asid [iff]:
-  "integrity aag X st (s\<lparr>arch_state := ((arch_state s)\<lparr>arm_next_asid := v\<rparr>)\<rparr>) = integrity aag X st s"
-  unfolding integrity_def
-  by (simp )
-
-declare dmo_mol_respects [wp]
-
-crunch respects[wp]: arm_context_switch "integrity X aag st"
-  (simp: dmo_bind_valid dsb_def isb_def writeTTBR0_def invalidateLocalTLB_ASID_def
-         setHardwareASID_def set_current_pd_def
- ignore: do_machine_op)
-
-crunch respects[wp]: set_vm_root "integrity X aag st"
-    (wp: crunch_wps
-   simp: set_current_pd_def isb_def dsb_def writeTTBR0_def dmo_bind_valid crunch_simps
- ignore: do_machine_op)
-
-crunch respects[wp]: set_vm_root_for_flush "integrity X aag st"
-  (wp: crunch_wps simp: set_current_pd_def crunch_simps ignore: do_machine_op)
-
-crunch respects[wp]: flush_table "integrity X aag st"
-  (wp: crunch_wps simp: invalidateLocalTLB_ASID_def crunch_simps ignore: do_machine_op)
-
-crunch respects[wp]: page_table_mapped "integrity X aag st"
-
-lemma kheap_eq_state_vrefsD:
-  "kheap s p = Some ko \<Longrightarrow> state_vrefs s p = vs_refs_no_global_pts ko"
-  by (simp add: state_vrefs_def)
-
-lemma kheap_eq_state_vrefs_pas_refinedD:
-  "\<lbrakk> kheap s p = Some ko;
-       (p', r, a) \<in> vs_refs_no_global_pts ko; pas_refined aag s \<rbrakk>
-    \<Longrightarrow> (pasObjectAbs aag p, a, pasObjectAbs aag p') \<in> pasPolicy aag"
-  apply (drule kheap_eq_state_vrefsD)
-  apply (erule pas_refined_mem[OF sta_vref, rotated])
-  apply simp
-  done
-
-lemma find_pd_for_asid_authority1:
-  "\<lbrace>pas_refined aag\<rbrace>
-      find_pd_for_asid asid
-   \<lbrace>\<lambda>pd s. (pasASIDAbs aag asid, Control, pasObjectAbs aag pd) \<in> pasPolicy aag\<rbrace>,-"
-  apply (rule hoare_pre)
-   apply (simp add: find_pd_for_asid_def)
-   apply (wp | wpc)+
-  apply (clarsimp simp: obj_at_def pas_refined_def)
-  apply (erule subsetD, erule sata_asid_lookup)
-  apply (simp add: state_vrefs_def vs_refs_no_global_pts_def image_def)
-  apply (rule rev_bexI, erule graph_ofI)
-  apply (simp add: mask_asid_low_bits_ucast_ucast)
-  done
-
-lemma find_pd_for_asid_authority2:
-  "\<lbrace>\<lambda>s. \<forall>pd. (\<forall>aag. pas_refined aag s \<longrightarrow> (pasASIDAbs aag asid, Control, pasObjectAbs aag pd) \<in> pasPolicy aag)
-           \<and> (pspace_aligned s \<and> valid_vspace_objs s \<longrightarrow> is_aligned pd pd_bits)
-           \<and> (\<exists>\<rhd> pd) s
-           \<longrightarrow> Q pd s\<rbrace> find_pd_for_asid asid \<lbrace>Q\<rbrace>, -"
-  (is "\<lbrace>?P\<rbrace> ?f \<lbrace>Q\<rbrace>,-")
-  apply (clarsimp simp: validE_R_def validE_def valid_def imp_conjL[symmetric])
-  apply (frule in_inv_by_hoareD[OF find_pd_for_asid_inv], clarsimp)
-  apply (drule spec, erule mp)
-  apply (simp add: use_validE_R[OF _ find_pd_for_asid_authority1]
-                   use_validE_R[OF _ find_pd_for_asid_aligned_pd_bits]
-                   use_validE_R[OF _ find_pd_for_asid_lookup])
-  done
-
-lemma find_pd_for_asid_pd_slot_authorised [wp]:
-  "\<lbrace>pas_refined aag and K (is_subject_asid aag asid) and pspace_aligned and valid_vspace_objs\<rbrace>
-  find_pd_for_asid asid
-  \<lbrace>\<lambda>rv s. is_subject aag (lookup_pd_slot rv vptr && ~~ mask pd_bits) \<rbrace>, -"
-  apply (wp find_pd_for_asid_authority2)
-  apply (clarsimp simp: lookup_pd_slot_pd)
-  apply (fastforce dest: pas_refined_Control)
-  done
-
-lemma unmap_page_table_respects:
-  "\<lbrace>integrity aag X st and pas_refined aag and invs
-         and K (is_subject_asid aag asid \<and> vaddr < kernel_base)\<rbrace>
-     unmap_page_table asid vaddr pt
-   \<lbrace>\<lambda>rv. integrity aag X st\<rbrace>"
-  apply (rule hoare_gen_asm)
-  apply (simp add: unmap_page_table_def page_table_mapped_def )
-  apply (rule hoare_pre)
-   apply (wp store_pde_respects page_table_mapped_wp_weak get_pde_wp
-             hoare_vcg_all_lift_R dmo_mol_respects
-        | wpc
-        | simp add: cleanByVA_PoU_def
-        | wp (once) hoare_drop_imps)+
-  apply auto
-  done
-
-definition
-  authorised_page_table_inv :: "'a PAS \<Rightarrow> page_table_invocation \<Rightarrow> bool"
-where
-  "authorised_page_table_inv aag pti \<equiv> case pti of
-     page_table_invocation.PageTableMap cap cslot_ptr pde obj_ref \<Rightarrow>
-         is_subject aag (fst cslot_ptr) \<and> is_subject aag (obj_ref && ~~ mask pd_bits)
-       \<and> (case_option True (is_subject aag o fst) (pde_ref2 pde))
-       \<and> pas_cap_cur_auth aag cap
-   | page_table_invocation.PageTableUnmap cap cslot_ptr \<Rightarrow>
-       is_subject aag (fst cslot_ptr) \<and> aag_cap_auth aag (pasSubject aag) cap
-         \<and> (\<forall>p asid vspace_ref. cap = cap.ArchObjectCap (arch_cap.PageTableCap p (Some (asid, vspace_ref)))
-                \<longrightarrow> is_subject_asid aag asid
-                \<and> (\<forall>x \<in> set [p , p + 4 .e. p + 2 ^ pt_bits - 1]. is_subject aag (x && ~~ mask pt_bits)))"
-
-lemma perform_page_table_invocation_respects:
-  "\<lbrace>integrity aag X st and pas_refined aag and invs
-          and valid_pti page_table_invocation
-          and K (authorised_page_table_inv aag page_table_invocation)\<rbrace>
-     perform_page_table_invocation page_table_invocation
-   \<lbrace>\<lambda>s. integrity aag X st\<rbrace>"
-  apply (rule hoare_gen_asm)
-  apply (simp add: perform_page_table_invocation_def
-             cong: page_table_invocation.case_cong option.case_cong prod.case_cong
-                   cap.case_cong arch_cap.case_cong)
-  apply (rule hoare_pre)
-  apply (wp store_pde_respects set_cap_integrity_autarch store_pte_respects unmap_page_table_respects mapM_wp'
-       | wpc
-       | simp add: mapM_x_mapM authorised_page_table_inv_def cleanByVA_PoU_def)+
-  apply (auto simp: cap_auth_conferred_def is_page_cap_def
-                    pas_refined_all_auth_is_owns
-                    valid_pti_def valid_cap_simps)
-  done
-
-crunch arm_asid_table_inv [wp]: unmap_page_table "\<lambda>s. P (arm_asid_table (arch_state s))"
- (wp: crunch_wps simp: crunch_simps)
-
-lemma clas_update_map_data_strg:
-  "(is_pg_cap cap \<or> is_pt_cap cap) \<longrightarrow> cap_links_asid_slot aag p (cap.ArchObjectCap (update_map_data (the_arch_cap cap) None))"
-  unfolding cap_links_asid_slot_def
-  by (fastforce simp: is_cap_simps update_map_data_def)
-
-lemmas pte_ref_simps = pte_ref_def[split_simps pte.split]
-
-lemmas store_pde_pas_refined_simple
-    = store_pde_pas_refined[where pde=InvalidPDE, simplified pde_ref_simps, simplified]
-
-crunch pas_refined[wp]: unmap_page_table "pas_refined aag"
-  (wp: crunch_wps store_pde_pas_refined_simple
-      simp: crunch_simps pde_ref_simps)
-
-lemma pde_ref_pde_ref2:
-  "\<lbrakk> pde_ref x = Some v; pde_ref2 x = Some v' \<rbrakk> \<Longrightarrow> v' = (v, 0, {Control})"
-  unfolding pde_ref_def pde_ref2_def
-  by (cases x, simp_all)
-
-lemma ptr_range_0 [simp]: "ptr_range (p :: word32) 0 = {p}"
-  unfolding ptr_range_def by simp
-
-lemma mask_PTCap_eq:
-  "(ArchObjectCap (PageTableCap a b) = mask_cap R cap) = (cap = ArchObjectCap (PageTableCap a b))"
-  by (auto simp: mask_cap_def cap_rights_update_def acap_rights_update_def
-           split: arch_cap.splits cap.splits bool.splits)
-
-
-(* FIXME MOVE *)
-crunch cdt[wp]: unmap_page_table "\<lambda>s. P (cdt s)"
-  (simp: crunch_simps wp: crunch_wps)
-
-(* FIXME MOVE *)
 lemma is_transferable_ArchCap[simp]:
-  "\<not> is_transferable
-        (Some (ArchObjectCap cap))"
+  "\<not> is_transferable (Some (ArchObjectCap cap))"
   using is_transferable.simps by simp
-
-
-
-lemma is_transferable_is_arch_update:
-  "is_arch_update cap cap' \<Longrightarrow> is_transferable (Some cap) = is_transferable (Some cap')"
-  using is_transferable.simps is_arch_cap_def is_arch_update_def cap_master_cap_def
-  by (simp split: cap.splits arch_cap.splits)
-
-lemma perform_page_table_invocation_pas_refined [wp]:
-  "\<lbrace> pas_refined aag and valid_pti page_table_invocation
-     and K (authorised_page_table_inv aag page_table_invocation)\<rbrace>
-     perform_page_table_invocation page_table_invocation
-   \<lbrace>\<lambda>s. pas_refined aag\<rbrace>"
-  apply (rule hoare_gen_asm)
-  apply (simp add: perform_page_table_invocation_def
-             cong: page_table_invocation.case_cong option.case_cong prod.case_cong
-                   cap.case_cong arch_cap.case_cong)
-  apply (rule hoare_pre)
-  apply (wp get_cap_wp mapM_wp' store_pte_cte_wp_at do_machine_op_cte_wp_at
-            hoare_vcg_all_lift set_cap_pas_refined_not_transferable
-        | (wp hoare_vcg_imp_lift, unfold disj_not1)
-        | wpc
-        | simp add: mapM_x_mapM authorised_page_table_inv_def imp_conjR
-                    pte_ref_simps
-        | wps
-        | blast)+
-  apply (cases page_table_invocation)
-   apply (fastforce simp: cte_wp_at_caps_of_state Option.is_none_def
-                          is_transferable_is_arch_update[symmetric]
-                          valid_pti_def is_cap_simps pas_refined_refl auth_graph_map_def2
-                    dest: pde_ref_pde_ref2)
-  apply (rename_tac s pt_cap page_cslot)
-  apply (case_tac page_cslot)
-  apply (rename_tac page_ptr page_slot)
-  apply (case_tac "\<exists>pt_ptr mapping. pt_cap = ArchObjectCap (PageTableCap pt_ptr mapping)")
-   prefer 2
-   apply fastforce
-  apply (elim exE)
-  apply clarsimp
-  apply (rename_tac page_cap)
-  apply (subgoal_tac
-            "cte_wp_at ((=) page_cap) (page_ptr, page_slot) s \<longrightarrow>
-             cte_wp_at (\<lambda>c. \<not> is_transferable (Some c)) (page_ptr, page_slot) s \<and>
-             pas_cap_cur_auth aag
-                (cap.ArchObjectCap (update_map_data (the_arch_cap page_cap) None))")
-   apply simp
-  apply (clarsimp simp: cte_wp_at_caps_of_state)
-  apply (frule (1) cap_cur_auth_caps_of_state)
-   apply simp
-  apply (clarsimp simp: valid_pti_def cte_wp_at_caps_of_state mask_PTCap_eq)
-  apply (clarsimp simp: cap_auth_conferred_def update_map_data_def is_page_cap_def
-                        cap_links_asid_slot_def cap_links_irq_def aag_cap_auth_def)
-  done
-
-definition
-  authorised_slots :: "'a PAS \<Rightarrow> pte \<times> (obj_ref list) + pde \<times> (obj_ref list) \<Rightarrow> bool"
-where
- "authorised_slots aag m \<equiv> case m of
-    Inl (pte, slots) \<Rightarrow> (\<forall>x. pte_ref pte = Some x \<longrightarrow> (\<forall>a \<in> (snd (snd x)). \<forall>p \<in> ptr_range (fst x) (fst (snd x)).(aag_has_auth_to aag a p)))
-           \<and> (\<forall>x \<in> set slots. is_subject aag (x && ~~ mask pt_bits))
-  | Inr (pde, slots) \<Rightarrow> (\<forall>x. pde_ref2 pde = Some x \<longrightarrow> (\<forall>a \<in> (snd (snd x)). \<forall>p \<in> ptr_range (fst x) (fst (snd x)). (aag_has_auth_to aag a p)))
-           \<and> (\<forall>x \<in> set slots. is_subject aag (x && ~~ mask pd_bits))"
-
-definition
-  authorised_page_inv :: "'a PAS \<Rightarrow> page_invocation \<Rightarrow> bool"
-where
-  "authorised_page_inv aag pgi \<equiv> case pgi of
-     PageMap asid cap ptr slots \<Rightarrow>
-       pas_cap_cur_auth aag cap \<and> is_subject aag (fst ptr) \<and> authorised_slots aag slots
-   | PageUnmap cap ptr \<Rightarrow> pas_cap_cur_auth aag (Structures_A.ArchObjectCap cap) \<and> is_subject aag (fst ptr)
-   | PageFlush typ start end pstart pd asid \<Rightarrow> True
-   | PageGetAddr ptr \<Rightarrow> True"
-
-crunch respects[wp]: lookup_pt_slot "integrity X aag st"
-
-lemma ptrFromPAddr_inj: "inj ptrFromPAddr"
-  by (auto intro: injI simp: ptrFromPAddr_def)
-
-lemma vs_refs_no_global_pts_pdI:
-  "\<lbrakk>pd (ucast r) = PageTablePDE x a b;
-    ((ucast r)::12 word) < ucast (kernel_base >> 20) \<rbrakk> \<Longrightarrow>
-        (ptrFromPAddr x, VSRef (r && mask 12)
-                  (Some APageDirectory), Control)
-          \<in> vs_refs_no_global_pts (ArchObj (PageDirectory pd))"
-  apply(clarsimp simp: vs_refs_no_global_pts_def)
-  apply (drule_tac f=pde_ref2 in arg_cong, simp add: pde_ref_simps o_def)
-  apply (rule rev_bexI, rule DiffI, erule graph_ofI)
-   apply simp
-  apply (clarsimp simp: ucast_ucast_mask )
-  done
-
-lemma aag_has_auth_to_Control_eq_owns:
-  "pas_refined aag s \<Longrightarrow> aag_has_auth_to aag Control p = is_subject aag p"
-  by (auto simp: pas_refined_refl elim: aag_Control_into_owns)
-
-lemma lookup_pt_slot_authorised:
-  "\<lbrace>\<exists>\<rhd> pd and valid_vspace_objs and pspace_aligned and pas_refined aag
-            and K (is_subject aag pd) and K (is_aligned pd 14 \<and> vptr < kernel_base)\<rbrace>
-    lookup_pt_slot pd vptr
-  \<lbrace>\<lambda>rv s. is_subject aag (rv && ~~ mask pt_bits)\<rbrace>, -"
-  apply (simp add: lookup_pt_slot_def)
-  apply (wp get_pde_wp | wpc)+
-  apply (subgoal_tac "is_aligned pd pd_bits")
-   apply (clarsimp simp: lookup_pd_slot_pd)
-   apply (drule(2) valid_vspace_objsD)
-   apply (clarsimp simp: obj_at_def)
-   apply (drule kheap_eq_state_vrefs_pas_refinedD)
-     apply (erule vs_refs_no_global_pts_pdI)
-     apply (drule(1) less_kernel_base_mapping_slots)
-     apply (simp add: kernel_mapping_slots_def)
-    apply assumption
-   apply (simp add: aag_has_auth_to_Control_eq_owns)
-   apply (drule_tac f="\<lambda>pde. valid_pde pde s" in arg_cong, simp)
-   apply (clarsimp simp: obj_at_def less_kernel_base_mapping_slots)
-   apply (erule pspace_alignedE, erule domI)
-   apply (simp add: pt_bits_def pageBits_def)
-   apply (subst is_aligned_add_helper, assumption)
-    apply (rule shiftl_less_t2n)
-     apply (rule order_le_less_trans, rule word_and_le1, simp)
-    apply simp
-   apply simp
-  apply (simp add: pd_bits_def pageBits_def)
-  done
-
-lemma is_aligned_6_masks:
-  fixes p :: word32
-  shows
-  "\<lbrakk> is_aligned p 6; bits = pt_bits \<or> bits = pd_bits \<rbrakk>
-        \<Longrightarrow> \<forall>x \<in> set [0, 4 .e. 0x3C]. x + p && ~~ mask bits = p && ~~ mask bits"
-  apply clarsimp
-  apply (drule subsetD[OF upto_enum_step_subset])
-  apply (subst mask_lower_twice[symmetric, where n=6])
-   apply (auto simp add: pt_bits_def pageBits_def pd_bits_def)[1]
-  apply (subst add.commute, subst is_aligned_add_helper, assumption)
-   apply (simp add: order_le_less_trans)
-  apply simp
-  done
-
-lemma lookup_pt_slot_authorised2:
-  "\<lbrace>\<exists>\<rhd> pd and K (is_subject aag pd) and
-    K (is_aligned pd 14 \<and> is_aligned vptr 16 \<and> vptr < kernel_base) and
-    valid_vspace_objs and valid_arch_state and equal_kernel_mappings and
-    valid_global_objs and pspace_aligned and pas_refined aag\<rbrace>
-    lookup_pt_slot pd vptr
-  \<lbrace>\<lambda>rv s.  \<forall>x\<in>set [0 , 4 .e. 0x3C]. is_subject aag (x + rv && ~~ mask pt_bits)\<rbrace>, -"
-  apply (clarsimp simp: validE_R_def valid_def validE_def
-                 split: sum.split)
-  apply (frule use_validE_R[OF _ lookup_pt_slot_authorised])
-   apply fastforce
-  apply (frule use_validE_R[OF _ lookup_pt_slot_is_aligned_6])
-   apply (fastforce simp add: vmsz_aligned_def pd_bits_def pageBits_def)
-  apply (simp add: is_aligned_6_masks)
-  done
-
-lemma lookup_pt_slot_authorised3:
-  "\<lbrace>\<exists>\<rhd> pd and K (is_subject aag pd) and
-    K (is_aligned pd 14 \<and> is_aligned vptr 16 \<and> vptr < kernel_base) and
-    valid_vspace_objs and valid_arch_state and equal_kernel_mappings and
-    valid_global_objs and pspace_aligned and pas_refined aag\<rbrace>
-    lookup_pt_slot pd vptr
-  \<lbrace>\<lambda>rv s.  \<forall>x\<in>set [rv , rv + 4 .e. rv + 0x3C]. is_subject aag (x && ~~ mask pt_bits)\<rbrace>, -"
-  apply (rule hoare_post_imp_R [where Q' = "\<lambda>rv s. is_aligned rv 6 \<and> (\<forall>x\<in>set [0 , 4 .e. 0x3C]. is_subject aag (x + rv && ~~ mask pt_bits))"])
-  apply (rule hoare_pre)
-  apply (wp lookup_pt_slot_is_aligned_6 lookup_pt_slot_authorised2)
-   apply (fastforce simp: vmsz_aligned_def pd_bits_def pageBits_def)
-  apply simp
-  apply (simp add: p_0x3C_shift)
-  done
 
 lemma mapM_set':
   assumes ip: "\<And>x y. \<lbrakk> x \<in> set xs; y \<in> set xs \<rbrakk> \<Longrightarrow> \<lbrace>I x and I y\<rbrace> f x \<lbrace>\<lambda>_. I y\<rbrace>"
-  and   rl: "\<And>s. (\<forall>x \<in> set xs. I x s) \<Longrightarrow> P s"
+  and rl: "\<And>s. (\<forall>x \<in> set xs. I x s) \<Longrightarrow> P s"
   shows "\<lbrace>\<lambda>s. (\<forall>x \<in> set xs. I x s)\<rbrace> mapM f xs \<lbrace>\<lambda>_. P\<rbrace>"
-  apply (rule hoare_post_imp [OF rl])
+  apply (rule hoare_post_imp[OF rl])
    apply assumption
   apply (rule mapM_set)
     apply (rule hoare_pre)
@@ -406,905 +54,166 @@ lemma mapM_set':
 
 lemma mapM_set'':
   assumes ip: "\<And>x y. \<lbrakk> x \<in> set xs; y \<in> set xs \<rbrakk> \<Longrightarrow> \<lbrace>I x and I y and Q\<rbrace> f x \<lbrace>\<lambda>_. I y and Q\<rbrace>"
-  and   rl: "\<And>s. (\<forall>x \<in> set xs. I x s) \<and> Q s \<Longrightarrow> P s"
+  and rl: "\<And>s. (\<forall>x \<in> set xs. I x s) \<and> Q s \<Longrightarrow> P s"
   shows "\<lbrace>\<lambda>s. (\<forall>x \<in> set xs. I x s) \<and> Q s\<rbrace> mapM f xs \<lbrace>\<lambda>_. P\<rbrace>"
-  apply (rule hoare_post_imp [OF rl])
+  apply (rule hoare_post_imp[OF rl])
    apply assumption
   apply (cases "xs = []")
    apply (simp add: mapM_Nil)
   apply (rule hoare_pre)
-   apply (rule mapM_set' [where I = "\<lambda>x s. I x s \<and> Q s"])
+   apply (rule mapM_set'[where I = "\<lambda>x s. I x s \<and> Q s"])
     apply (rule hoare_pre)
-     apply (rule ip [simplified pred_conj_def])
-      apply simp_all
-  apply (clarsimp simp add: neq_Nil_conv)
+     apply (rule ip[simplified pred_conj_def])
+      apply (auto simp: neq_Nil_conv)
   done
 
-crunch respects [wp]: flush_page "integrity aag X st"
-  (simp: invalidateLocalTLB_VAASID_def ignore: do_machine_op)
-
-lemma find_pd_for_asid_pd_owned[wp]:
-  "\<lbrace>pas_refined aag and K (is_subject_asid aag asid)\<rbrace>
-  find_pd_for_asid asid
-  \<lbrace>\<lambda>rv s. is_subject aag rv\<rbrace>,-"
-  apply (wp find_pd_for_asid_authority2)
-  apply (auto simp: aag_has_auth_to_Control_eq_owns)
-  done
-
-lemmas store_pte_pas_refined_simple
-   = store_pte_pas_refined[where pte=InvalidPTE, simplified pte_ref_simps, simplified]
-
-crunch pas_refined[wp]: unmap_page "pas_refined aag"
-  (wp: crunch_wps store_pde_pas_refined_simple store_pte_pas_refined_simple
-       simp: crunch_simps)
-
-lemma unmap_page_respects:
-  "\<lbrace>integrity aag X st and K (is_subject_asid aag asid) and pas_refined aag and pspace_aligned and valid_vspace_objs
-        and K (vmsz_aligned vptr sz \<and> vptr < kernel_base)\<rbrace>
-    unmap_page sz asid vptr pptr
-   \<lbrace>\<lambda>rv. integrity aag X st\<rbrace>"
-  apply (rule hoare_gen_asm)
-  apply (simp add: unmap_page_def swp_def cong: vmpage_size.case_cong)
+lemma as_user_pas_refined[wp]:
+  "as_user t f \<lbrace>pas_refined aag\<rbrace>"
+  apply (simp add: pas_refined_def state_objs_to_policy_def)
   apply (rule hoare_pre)
-   apply (wp store_pte_respects store_pde_respects
-             hoare_drop_imps[where Q="\<lambda>rv. integrity aag X st"]
-             lookup_pt_slot_authorised
-                   | wpc
-                   | simp add: is_aligned_6_masks is_aligned_mask[symmetric] cleanByVA_PoU_def
-                   | wp (once) hoare_drop_imps
-                     mapM_set'' [where f = "(\<lambda>a. store_pte a InvalidPTE)" and I = "\<lambda>x s. is_subject aag (x && ~~ mask pt_bits)" and Q = "integrity aag X st"]
-                     mapM_set'' [where f = "(\<lambda>a. store_pde a InvalidPDE)" and I = "\<lambda>x s. is_subject aag (x && ~~ mask pd_bits)" and Q = "integrity aag X st"]
-                   | wp (once) hoare_drop_imps[where R="\<lambda>rv s. rv"])+
-  done
-
-(* FIXME: MOVE *)
-lemma less_shiftr:
-  shows "\<lbrakk> x < y; is_aligned y n \<rbrakk> \<Longrightarrow> x >> n < y >> n"
-  apply (simp add: word_less_nat_alt shiftr_div_2n')
-  apply (subst td_gal_lt[symmetric])
-   apply simp
-  apply (subst dvd_div_mult_self)
-   apply (simp add: is_aligned_def)
+   apply wps
+   apply wp
   apply simp
   done
 
-lemma kernel_base_aligned_20:
-  "is_aligned kernel_base 20"
-  apply(simp add: kernel_base_def is_aligned_def)
-  done
+crunches set_message_info
+  for pas_refined[wp]: "pas_refined aag"
+  and cdt[wp]: "\<lambda>s. P (cdt s)"
 
-(* FIXME: CLAG *)
-lemmas do_machine_op_bind =
-    submonad_bind [OF submonad_do_machine_op submonad_do_machine_op
-                      submonad_do_machine_op]
+crunches do_machine_op
+  for thread_states[wp]: "\<lambda>s. P (thread_states s)"
+  and state_vrefs[wp]: "\<lambda>s :: 'a :: state_ext state. P (state_vrefs s)"
 
-lemma mol_mem[wp]:
-  "\<lbrace>\<lambda>ms. P (underlying_memory ms)\<rbrace> machine_op_lift mop \<lbrace>\<lambda>rv ms. P (underlying_memory ms)\<rbrace>"
-  by (simp add: machine_op_lift_def machine_rest_lift_def split_def | wp)+
-
-lemma mol_dvs[wp]:
-  "\<lbrace>\<lambda>ms. P (device_state ms)\<rbrace> machine_op_lift mop \<lbrace>\<lambda>rv ms. P (device_state ms)\<rbrace>"
-  by (simp add: machine_op_lift_def machine_rest_lift_def split_def | wp)+
-
-lemmas do_flush_defs = cleanCacheRange_RAM_def cleanCacheRange_PoC_def cleanCacheRange_PoU_def invalidateCacheRange_RAM_def cleanInvalidateCacheRange_RAM_def branchFlushRange_def invalidateCacheRange_I_def
-
-lemma do_flush_respects[wp]:
-  "\<lbrace>integrity aag X st\<rbrace> do_machine_op (do_flush typ start end pstart)
-    \<lbrace>\<lambda>rv. integrity aag X st\<rbrace>"
-  apply (cases "typ")
-     apply (wp dmo_no_mem_respects | simp add: do_flush_def cache_machine_op_defs do_flush_defs)+
-     done
-
-lemma invalidate_tlb_by_asid_respects[wp]:
-  "\<lbrace>integrity aag X st\<rbrace> invalidate_tlb_by_asid asid
-    \<lbrace>\<lambda>rv. integrity aag X st\<rbrace>"
-  apply (simp add: invalidate_tlb_by_asid_def)
-  apply (wp dmo_no_mem_respects | wpc | simp add: invalidateLocalTLB_ASID_def )+
-  done
-
-lemma invalidate_tlb_by_asid_pas_refined[wp]:
-  "\<lbrace>pas_refined aag\<rbrace> invalidate_tlb_by_asid asid \<lbrace>\<lambda>rv. pas_refined aag\<rbrace>"
-  by (wp dmo_no_mem_respects | wpc | simp add: invalidate_tlb_by_asid_def invalidateLocalTLB_ASID_def)+
-
-crunch pas_refined[wp]: set_message_info "pas_refined aag"
-
-(* FIXME: move *)
-lemma set_message_info_mdb[wp]:
-  "\<lbrace>\<lambda>s. P (cdt s)\<rbrace> set_message_info thread info \<lbrace>\<lambda>rv s. P (cdt s)\<rbrace>"
-  unfolding set_message_info_def by wp
-
-crunch state_vrefs[wp]: do_machine_op "\<lambda>s::'z::state_ext state. P (state_vrefs s)"
-
-crunch thread_states[wp]: do_machine_op "\<lambda>s. P (thread_states s)"
-
-(* FIXME: move *)
-lemma set_mrs_state_vrefs[wp]:
-  "\<lbrace>\<lambda>s. P (state_vrefs s)\<rbrace> set_mrs thread buf msgs \<lbrace>\<lambda>rv s. P (state_vrefs s)\<rbrace>"
-  apply (simp add: set_mrs_def split_def set_object_def get_object_def split del: if_split)
-  apply (wp gets_the_wp get_wp put_wp mapM_x_wp'
-       | wpc
-       | simp split del: if_split add: zipWithM_x_mapM_x split_def store_word_offs_def)+
-  apply (auto simp: obj_at_def state_vrefs_def get_tcb_ko_at
-             elim!: rsubst[where P=P, OF _ ext]
-             split: if_split_asm simp: vs_refs_no_global_pts_def)
-  done
+crunch integrity_autarch: set_message_info "integrity aag X st"
 
 (* FIXME: move *)
 lemma set_mrs_thread_states[wp]:
-  "\<lbrace>\<lambda>s. P (thread_states s)\<rbrace> set_mrs thread buf msgs \<lbrace>\<lambda>rv s. P (thread_states s)\<rbrace>"
-  apply (simp add: set_mrs_def split_def set_object_def get_object_def split del: if_split)
-  apply (wp gets_the_wp get_wp put_wp mapM_x_wp'
-       | wpc
-       | simp split del: if_split add: zipWithM_x_mapM_x split_def store_word_offs_def)+
+  "set_mrs thread buf msgs \<lbrace>\<lambda>s. P (thread_states s)\<rbrace>"
+  supply if_split[split del]
+  apply (simp add: set_mrs_def split_def set_object_def get_object_def)
+  apply (wpsimp wp: gets_the_wp get_wp put_wp mapM_x_wp'
+              simp: zipWithM_x_mapM_x split_def store_word_offs_def)
   apply (clarsimp simp: fun_upd_def[symmetric] thread_states_preserved)
   done
 
 lemma set_mrs_thread_bound_ntfns[wp]:
-  "\<lbrace>\<lambda>s. P (thread_bound_ntfns s)\<rbrace> set_mrs thread buf msgs \<lbrace>\<lambda>rv s. P (thread_bound_ntfns s)\<rbrace>"
-  apply (simp add: set_mrs_def split_def set_object_def get_object_def split del: if_split)
-  apply (wp gets_the_wp get_wp put_wp mapM_x_wp' dmo_wp
-       | wpc
-       | simp split del: if_split add: zipWithM_x_mapM_x split_def store_word_offs_def no_irq_storeWord)+
-  apply (clarsimp simp: fun_upd_def[symmetric] thread_bound_ntfns_preserved )
+  "set_mrs thread buf msgs \<lbrace>\<lambda>s. P (thread_bound_ntfns s)\<rbrace>"
+  supply if_split[split del]
+  apply (simp add: set_mrs_def split_def set_object_def get_object_def )
+  apply (wpsimp wp: gets_the_wp get_wp put_wp mapM_x_wp' dmo_wp
+              simp: zipWithM_x_mapM_x split_def store_word_offs_def no_irq_storeWord)
+  apply (clarsimp simp: fun_upd_def[symmetric] thread_bound_ntfns_preserved)
+  done
+
+lemma delete_objects_pspace_no_overlap:
+  "\<lbrace>pspace_aligned and valid_objs and (\<lambda>s. \<exists>idx. cte_wp_at ((=) (UntypedCap dev ptr sz idx)) slot s)\<rbrace>
+   delete_objects ptr sz
+   \<lbrace>\<lambda>_. pspace_no_overlap_range_cover ptr sz\<rbrace>"
+  unfolding delete_objects_def do_machine_op_def
+  apply (wp | simp add: split_def detype_machine_state_update_comm)+
+  apply (clarsimp)
+  apply (rule pspace_no_overlap_detype)
+    apply (auto dest: cte_wp_at_valid_objs_valid_cap)
+  done
+
+lemma delete_objects_invs_ex:
+  "\<lbrace>invs and ct_active and
+    (\<lambda>s. \<exists>slot dev f. cte_wp_at ((=) (UntypedCap dev ptr bits f)) slot s \<and>
+                      descendants_range (UntypedCap dev ptr bits f) slot s)\<rbrace>
+   delete_objects ptr bits
+   \<lbrace>\<lambda>_. invs\<rbrace>"
+  apply (clarsimp simp: valid_def)
+  apply (erule use_valid)
+   apply wp
+  apply auto
+  done
+
+lemma is_subject_asid_into_loas:
+  "\<lbrakk> is_subject_asid aag asid; pas_refined aag s \<rbrakk>
+     \<Longrightarrow> label_owns_asid_slot aag (pasSubject aag) asid"
+  unfolding label_owns_asid_slot_def
+  by (clarsimp simp: pas_refined_refl)
+
+
+locale Arch_AC_1 =
+  assumes set_mrs_state_vrefs[wp]:
+    "set_mrs thread buf msgs \<lbrace>\<lambda>s :: det_ext state. P (state_vrefs s)\<rbrace>"
+  and mul_add_word_size_lt_msg_align_bits_ofnat:
+    "\<lbrakk> p < 2 ^ (msg_align_bits - word_size_bits); k < 4 \<rbrakk>
+       \<Longrightarrow> of_nat p * of_nat word_size + k < (2 :: obj_ref) ^ msg_align_bits"
+begin
+
+lemmas mul_word_size_lt_msg_align_bits_ofnat =
+  mul_add_word_size_lt_msg_align_bits_ofnat[where k=0, simplified]
+
+lemmas ptr_range_off_off_mems =
+  ptr_range_add_memI[OF _ mul_word_size_lt_msg_align_bits_ofnat]
+  ptr_range_add_memI[OF _ mul_add_word_size_lt_msg_align_bits_ofnat, simplified add.assoc[symmetric]]
+
+lemma dmo_storeWord_respects_Write:
+  "\<lbrace>integrity aag X st and K (\<forall>p' \<in> ptr_range p word_size_bits. aag_has_auth_to aag Write p')\<rbrace>
+   do_machine_op (storeWord p v)
+   \<lbrace>\<lambda>_. integrity aag X st\<rbrace>"
+  apply (rule hoare_pre)
+  apply (wp dmo_wp storeWord_respects)
+  apply simp
+  done
+
+lemma store_word_offs_integrity_autarch:
+  "\<lbrace>\<lambda>s. integrity aag X st s \<and> is_subject aag thread \<and>
+        ipc_buffer_has_auth aag thread (Some buf) \<and>
+        r < 2 ^ (msg_align_bits - word_size_bits)\<rbrace>
+   store_word_offs buf r v
+   \<lbrace>\<lambda>_. integrity aag X st\<rbrace>"
+  apply (simp add: store_word_offs_def)
+  apply (rule hoare_pre)
+   apply (wp dmo_storeWord_respects_Write)
+  apply clarsimp
+  apply (drule (1) ipc_buffer_has_auth_wordE)
+     apply (simp add: word_size_word_size_bits is_aligned_mult_triv2)
+    apply (simp add: msg_align_bits')
+   apply (erule mul_word_size_lt_msg_align_bits_ofnat)
+  apply simp
   done
 
 lemma set_mrs_pas_refined[wp]:
-  "\<lbrace>pas_refined aag\<rbrace> set_mrs thread buf msgs \<lbrace>\<lambda>rv. pas_refined aag\<rbrace>"
+  "set_mrs thread buf msgs \<lbrace>pas_refined aag\<rbrace>"
   apply (simp add: pas_refined_def state_objs_to_policy_def)
   apply (rule hoare_pre)
    apply (wp | wps)+
   apply (clarsimp dest!: auth_graph_map_memD)
   done
 
-crunch integrity_autarch: set_message_info "integrity aag X st"
-
-lemma dmo_storeWord_respects_Write:
-  "\<lbrace>integrity aag X st and K (\<forall>p' \<in> ptr_range p 2. aag_has_auth_to aag Write p')\<rbrace>
-  do_machine_op (storeWord p v)
-  \<lbrace>\<lambda>a. integrity aag X st\<rbrace>"
-  apply (rule hoare_pre)
-  apply (wp dmo_wp storeWord_respects)
-  apply simp
-  done
-
-(* c.f.  auth_ipc_buffers *)
-definition
-  ipc_buffer_has_auth :: "'a PAS \<Rightarrow> word32 \<Rightarrow> word32 option \<Rightarrow> bool"
-where
-   "ipc_buffer_has_auth aag thread \<equiv>
-    case_option True (\<lambda>buf'. is_aligned buf' msg_align_bits \<and> (\<forall>x \<in> ptr_range buf' msg_align_bits. (pasObjectAbs aag thread, Write, pasObjectAbs aag x) \<in> pasPolicy aag))"
-
-lemma ipc_buffer_has_auth_wordE:
-  "\<lbrakk> ipc_buffer_has_auth aag thread (Some buf); p \<in> ptr_range (buf + off) sz; is_aligned off sz; sz \<le> msg_align_bits; off < 2 ^ msg_align_bits \<rbrakk>
-  \<Longrightarrow> (pasObjectAbs aag thread, Write, pasObjectAbs aag p) \<in> pasPolicy aag"
-  unfolding ipc_buffer_has_auth_def
-  apply clarsimp
-  apply (erule bspec)
-  apply (erule (4) set_mp [OF ptr_range_subset])
-  done
-
-
-lemma is_aligned_word_size_2 [simp]:
-  "is_aligned (p * of_nat word_size) 2"
-  unfolding word_size_def
-  by (simp add: is_aligned_mult_triv2 [where n = 2, simplified] word_bits_conv)
-
-
-
-lemma mul_word_size_lt_msg_align_bits_ofnat:
-  "p < 2 ^ (msg_align_bits - 2) \<Longrightarrow> of_nat p * of_nat word_size < (2 :: word32) ^ msg_align_bits"
-  unfolding word_size_def
-  apply simp
-  apply (rule word_less_power_trans_ofnat [where k = 2, simplified])
-  apply (simp_all add: msg_align_bits word_bits_conv)
-  done
-
-lemma store_word_offs_integrity_autarch:
-  "\<lbrace>integrity aag X st and K (is_subject aag thread \<and> ipc_buffer_has_auth aag thread (Some buf) \<and> r < 2 ^ (msg_align_bits - 2))\<rbrace>
-   store_word_offs buf r v
-   \<lbrace>\<lambda>rv. integrity aag X st\<rbrace>"
-  apply (simp add: store_word_offs_def)
-  apply (rule hoare_pre)
-   apply (wp dmo_storeWord_respects_Write)
-  apply clarsimp
-  apply (drule (1) ipc_buffer_has_auth_wordE)
-     apply simp
-    apply (simp add: msg_align_bits)
-   apply (erule mul_word_size_lt_msg_align_bits_ofnat)
-  apply simp
+lemma copy_mrs_integrity_autarch:
+  "\<lbrace>pas_refined aag and integrity aag X st and
+    K (is_subject aag receiver \<and> ipc_buffer_has_auth aag receiver rbuf \<and>
+       unat n < 2 ^ (msg_align_bits - word_size_bits))\<rbrace>
+   copy_mrs sender sbuf receiver rbuf n
+   \<lbrace>\<lambda>_. integrity aag X st\<rbrace>"
+  apply (rule hoare_gen_asm)
+  apply (simp add: copy_mrs_def cong: if_cong split del: if_split)
+  apply (wpsimp wp: mapM_wp' as_user_integrity_autarch
+                    store_word_offs_integrity_autarch[where thread=receiver]
+         | fastforce)+
   done
 
 lemma set_mrs_integrity_autarch:
-  "\<lbrace>integrity aag X st and K (is_subject aag thread \<and>  ipc_buffer_has_auth aag thread buf)\<rbrace>
-     set_mrs thread buf msgs
-   \<lbrace>\<lambda>rv. integrity aag X st\<rbrace>"
+  "\<lbrace>integrity aag X st and K (is_subject aag thread \<and> ipc_buffer_has_auth aag thread buf)\<rbrace>
+   set_mrs thread buf msgs
+   \<lbrace>\<lambda>_. integrity aag X st\<rbrace>"
   apply (rule hoare_gen_asm)
   apply (simp add: set_mrs_def split del: if_split)
-  apply (wp gets_the_wp get_wp put_wp mapM_x_wp' store_word_offs_integrity_autarch [where aag = aag and thread = thread]
-       | wpc
-       | simp split del: if_split add: split_def zipWithM_x_mapM_x )+
-    apply (clarsimp elim!: in_set_zipE split: if_split_asm)
-    apply (rule order_le_less_trans [where y = msg_max_length])
-     apply (fastforce simp add: le_eq_less_or_eq)
-    apply (simp add: msg_max_length_def msg_align_bits)
-   apply simp
-   apply (wp set_object_integrity_autarch hoare_drop_imps hoare_vcg_all_lift)+
-  apply simp
-  done
-
-lemma perform_page_invocation_respects:
-  "\<lbrace>integrity aag X st and pas_refined aag and K (authorised_page_inv aag pgi) and valid_page_inv pgi and valid_vspace_objs and pspace_aligned and is_subject aag  \<circ> cur_thread\<rbrace>
-     perform_page_invocation pgi
-   \<lbrace>\<lambda>s. integrity aag X st\<rbrace>"
-proof -
-  (* does not work as elim rule with clarsimp, which hammers Ball in concl. *)
-  have set_tl_subset_mp: "\<And>xs a. a \<in> set (tl xs) \<Longrightarrow> a \<in> set xs" by (case_tac xs,clarsimp+)
-  have hd_valid_slots:
-    "\<And>a xs s. valid_slots (Inl (a, xs)) s \<Longrightarrow> hd xs \<in> set xs"
-    "\<And>a xs s. valid_slots (Inr (a, xs)) s \<Longrightarrow> hd xs \<in> set xs"
-    by (simp_all add: valid_slots_def)
-
-  show ?thesis
-  apply (simp add: perform_page_invocation_def mapM_discarded swp_def
-                   valid_page_inv_def valid_unmap_def
-                   authorised_page_inv_def authorised_slots_def
-            split: page_invocation.split sum.split
-                   arch_cap.split option.split,
-         safe)
-        apply (wp set_cap_integrity_autarch unmap_page_respects
-                  mapM_x_and_const_wp[OF store_pte_respects] store_pte_respects
-                  mapM_x_and_const_wp[OF store_pde_respects] store_pde_respects
-             | elim conjE hd_valid_slots[THEN bspec[rotated]]
-             | clarsimp dest!:set_tl_subset_mp
-             | wpc )+
-   apply (clarsimp simp: cte_wp_at_caps_of_state cap_auth_conferred_def cap_rights_update_def
-                         acap_rights_update_def update_map_data_def is_pg_cap_def
-                         valid_page_inv_def valid_cap_simps
-                  dest!: cap_master_cap_eqDs)
-   apply (drule (1) clas_caps_of_state)
-   apply (simp add: cap_links_asid_slot_def label_owns_asid_slot_def)
-   apply (auto dest: pas_refined_Control)[1]
-  apply (wp set_mrs_integrity_autarch set_message_info_integrity_autarch | simp add: ipc_buffer_has_auth_def)+
-  done
-qed
-
-(* FIXME MOVE *)
-crunch cdt[wp]: unmap_page "\<lambda>s. P (cdt s)"
-  (simp: crunch_simps wp: crunch_wps)
-
-
-lemma perform_page_invocation_pas_refined [wp]:
-  "\<lbrace>pas_refined aag and K (authorised_page_inv aag pgi) and valid_page_inv pgi\<rbrace>
-     perform_page_invocation pgi
-   \<lbrace>\<lambda>_. pas_refined aag\<rbrace>"
-  apply (simp add: perform_page_invocation_def mapM_discarded
-    valid_page_inv_def valid_unmap_def swp_def
-    authorised_page_inv_def authorised_slots_def
-    cong: page_invocation.case_cong sum.case_cong)
-  apply (rule hoare_pre)
-   apply wpc
-      apply (wp set_cap_pas_refined unmap_page_pas_refined case_sum_wp  case_prod_wp
-                mapM_x_and_const_wp [OF store_pte_pas_refined] mapM_x_and_const_wp [OF store_pde_pas_refined]
-             hoare_vcg_all_lift hoare_vcg_const_imp_lift get_cap_wp
-            | (wp hoare_vcg_imp_lift, unfold disj_not1)
-            | strengthen clas_update_map_data_strg
-            | wpc
-            | wps
-            | simp)+
-  apply (case_tac pgi)
-      apply ((force simp: valid_slots_def pte_ref_def cte_wp_at_caps_of_state
-                          is_transferable_is_arch_update[symmetric]
-                          pde_ref2_def auth_graph_map_mem pas_refined_refl
-                   split: sum.splits)+)[2]
-    apply (clarsimp simp: cte_wp_at_caps_of_state is_transferable_is_arch_update[symmetric]
-                          pte_ref_def pde_ref2_def is_cap_simps is_pg_cap_def cap_auth_conferred_def)
-    apply (frule(1) cap_cur_auth_caps_of_state, simp)
-    apply (intro impI conjI;
-           clarsimp; (* NB: for speed *)
-           clarsimp simp: update_map_data_def clas_no_asid aag_cap_auth_def
-                          cap_auth_conferred_def vspace_cap_rights_to_auth_def
-                          cli_no_irqs is_pg_cap_def
-                          pte_ref_def[simplified aag_cap_auth_def])+
-  done
-
-definition
-  authorised_asid_control_inv :: "'a PAS \<Rightarrow> asid_control_invocation \<Rightarrow> bool"
-where
- "authorised_asid_control_inv aag aci \<equiv> case aci of
-     asid_control_invocation.MakePool frame slot parent base \<Rightarrow>
-       is_subject aag (fst slot) \<and> is_aligned frame pageBits \<and> (\<forall>asid. is_subject_asid aag asid) \<and> is_subject aag (fst parent) \<and>
-       (\<forall>x \<in> {frame..frame + 2 ^ pageBits - 1}. is_subject aag x)"
-
-
-lemma integrity_arm_asid_table_entry_update':
-  "\<lbrakk>integrity aag X st s;  asid_table = arm_asid_table (arch_state s);
-       (\<forall>asid'.
-                    asid' \<noteq> 0 \<and>
-                    asid_high_bits_of asid' = asid_high_bits_of asid \<longrightarrow>
-                    is_subject_asid aag asid')\<rbrakk> \<Longrightarrow>
-       integrity aag X st
-           (s\<lparr>arch_state := arch_state s
-                \<lparr>arm_asid_table :=
-                   \<lambda>a. if a = asid_high_bits_of asid then v
-                       else asid_table a\<rparr>\<rparr>)"
-  apply(clarsimp simp: integrity_def integrity_asids_def)
-  done
-
-lemma arm_asid_table_entry_update_integrity[wp]:
- "\<lbrace>integrity aag X st and (\<lambda> s. asid_table = arm_asid_table (arch_state s)) and K (\<forall>asid'.
-                    asid' \<noteq> 0 \<and>
-                    asid_high_bits_of asid' = asid_high_bits_of asid \<longrightarrow>
-                    is_subject_asid aag asid')\<rbrace>
- modify
-        (\<lambda>s. s\<lparr>arch_state := arch_state s
-                 \<lparr>arm_asid_table := asid_table
-                    (asid_high_bits_of asid := v)\<rparr>\<rparr>)
-  \<lbrace>\<lambda>_. integrity aag X st\<rbrace>"
-  apply (wp| simp)+
-  apply (blast intro: integrity_arm_asid_table_entry_update')
-  done
-
-lemma perform_asid_control_invocation_respects:
-  "\<lbrace>integrity aag X st and K (authorised_asid_control_inv aag aci)\<rbrace>
-     perform_asid_control_invocation aci
-   \<lbrace>\<lambda>s. integrity aag X st\<rbrace>"
-  apply (simp add: perform_asid_control_invocation_def)
-  apply (rule hoare_pre)
-   apply (wpc, simp)
-   apply (wp set_cap_integrity_autarch cap_insert_integrity_autarch retype_region_integrity[where sz=12] static_imp_wp | simp)+
-  apply (clarsimp simp: authorised_asid_control_inv_def
-                        ptr_range_def page_bits_def add.commute
-                        range_cover_def obj_bits_api_def default_arch_object_def
-                        pageBits_def word_bits_def)
-  apply(subst is_aligned_neg_mask_eq[THEN sym], assumption)
-  apply(simp add: and_mask_eq_iff_shiftr_0 mask_zero)
-  done
-
-lemma pas_refined_set_asid_strg:
-  "pas_refined aag s \<and> is_subject aag pool \<and> (\<forall>asid. asid_high_bits_of asid = base \<longrightarrow> is_subject_asid aag asid)
-    \<longrightarrow>
-  pas_refined aag (s\<lparr>arch_state := arch_state s \<lparr>arm_asid_table := (arm_asid_table (arch_state s))(base \<mapsto> pool)\<rparr>\<rparr>)"
-  apply (clarsimp simp: pas_refined_def state_objs_to_policy_def)
-  apply (erule state_asids_to_policy_aux.cases, simp_all split: if_split_asm)
-    apply (auto intro: state_asids_to_policy_aux.intros auth_graph_map_memI[OF sbta_vref] pas_refined_refl[simplified pas_refined_def state_objs_to_policy_def])
-  done
-
-
-(* FIXME: copied from Detype_R. *)
-lemma gets_modify_comm2:
-  "\<forall>s. g (f s) = g s \<Longrightarrow>
-   (do x \<leftarrow> modify f; y \<leftarrow> gets g; m x y od) =
-   (do y \<leftarrow> gets g; x \<leftarrow> modify f; m x y od)"
-  apply (rule ext)
-  apply (drule spec)
-  by (rule gets_modify_comm)
-lemma dmo_detype_comm:
-  assumes "empty_fail f"
-  shows "do_machine_op f >>= (\<lambda>s. modify (detype S)) =
-         modify (detype S) >>= (\<lambda>s. do_machine_op f)"
-proof -
-  have machine_state_detype: "\<forall>s. machine_state (detype S s) = machine_state s"
-    by (simp add: detype_def)
-  have detype_msu_independent:
-    "\<And>f. detype S \<circ> machine_state_update f = machine_state_update f \<circ> detype S"
-    by (simp add: detype_def ext)
-  from assms
-  show ?thesis
-    apply (simp add: do_machine_op_def split_def bind_assoc)
-    apply (simp add: gets_modify_comm2[OF machine_state_detype])
-    apply (rule arg_cong_bind1)
-    apply (simp add: empty_fail_def select_f_walk[OF empty_fail_modify]
-                     modify_modify detype_msu_independent)
-    done
-qed
-
-(* FIXME: copied from Detype_R. *)
-lemma empty_fail_freeMemory: "empty_fail (freeMemory ptr bits)"
-  by (simp add: freeMemory_def mapM_x_mapM ef_storeWord)
-
-(* FIXME: copied from Detype_R. *)
-lemma delete_objects_def2:
-  "delete_objects ptr bits \<equiv>
-   do modify (detype {ptr..ptr + 2 ^ bits - 1});
-      do_machine_op (freeMemory ptr bits)
-   od"
-  by (rule eq_reflection)
-     (simp add: delete_objects_def dmo_detype_comm[OF empty_fail_freeMemory])
-
-lemma delete_objects_pspace_no_overlap:
-  "\<lbrace> pspace_aligned and valid_objs and
-     (\<lambda> s. \<exists> idx. cte_wp_at ((=) (UntypedCap dev ptr sz idx)) slot s)\<rbrace>
-    delete_objects ptr sz
-   \<lbrace>\<lambda>rv. pspace_no_overlap_range_cover ptr sz\<rbrace>"
-  unfolding delete_objects_def do_machine_op_def
-  apply(wp | simp add: split_def detype_machine_state_update_comm)+
-  apply(clarsimp)
-  apply(rule pspace_no_overlap_detype)
-   apply(auto dest: cte_wp_at_valid_objs_valid_cap)
-  done
-
-
-lemma delete_objects_invs_ex:
-  "\<lbrace>(\<lambda>s. \<exists>slot dev f.
-         cte_wp_at ((=) (UntypedCap dev ptr bits f)) slot s \<and>
-         descendants_range (UntypedCap dev ptr bits f) slot s) and
-   invs and
-   ct_active\<rbrace>
-  delete_objects ptr bits \<lbrace>\<lambda>_. invs\<rbrace>"
-  apply(clarsimp simp: valid_def)
-  apply(erule use_valid)
-  apply wp
-  apply auto
-  done
-
-
-lemma perform_asid_control_invocation_pas_refined [wp]:
-  notes delete_objects_invs[wp del]
-  shows
-  "\<lbrace>pas_refined aag and pas_cur_domain aag and invs and valid_aci aci and ct_active and
-    K (authorised_asid_control_inv aag aci)\<rbrace>
-   perform_asid_control_invocation aci
-   \<lbrace>\<lambda>_. pas_refined aag\<rbrace>"
-  apply (simp add: perform_asid_control_invocation_def)
-  apply (rule hoare_pre)
-   apply (wp cap_insert_pas_refined' static_imp_wp
-        | strengthen pas_refined_set_asid_strg
-        | wpc
-        | simp add: delete_objects_def2 fun_upd_def[symmetric])+
-      apply (wp retype_region_pas_refined'[where sz=pageBits]
-                hoare_vcg_ex_lift hoare_vcg_all_lift static_imp_wp hoare_wp_combs hoare_drop_imp
-                retype_region_invs_extras(4)[where sz = pageBits]
-            | simp add: do_machine_op_def split_def cte_wp_at_neg2)+
-      apply (wp retype_region_cte_at_other'[where sz=pageBits]
-                max_index_upd_invs_simple max_index_upd_caps_overlap_reserved
-                hoare_vcg_ex_lift set_cap_cte_wp_at hoare_vcg_disj_lift set_free_index_valid_pspace
-                set_cap_descendants_range_in set_cap_no_overlap get_cap_wp set_cap_caps_no_overlap
-                hoare_vcg_all_lift static_imp_wp retype_region_invs_extras
-                set_cap_pas_refined_not_transferable
-            | simp add: do_machine_op_def split_def cte_wp_at_neg2 region_in_kernel_window_def)+
-   apply (rename_tac frame slot parent base cap)
-   apply (case_tac slot, rename_tac slot_ptr slot_idx)
-   apply (case_tac parent, rename_tac parent_ptr parent_idx)
-   apply (rule_tac Q="\<lambda>rv s.
-             (\<exists>idx. cte_wp_at ((=) (UntypedCap False frame pageBits idx)) parent s) \<and>
-             (\<forall>x\<in>ptr_range frame pageBits. is_subject aag x) \<and>
-             pas_refined aag s \<and>
-             pas_cur_domain aag s \<and>
-             pspace_no_overlap_range_cover frame pageBits s \<and>
-             invs s \<and>
-             descendants_range_in
-               {frame..(frame && ~~ mask pageBits) + 2 ^ pageBits - 1} parent s \<and>
-             range_cover frame pageBits
-               (obj_bits_api (ArchObject ASIDPoolObj) 0) (Suc 0) \<and>
-             is_subject aag slot_ptr \<and>
-             is_subject aag parent_ptr \<and>
-             pas_cap_cur_auth aag (ArchObjectCap (ASIDPoolCap frame base)) \<and>
-             is_subject aag frame \<and>
-             (\<forall>x. asid_high_bits_of x = asid_high_bits_of base \<longrightarrow>
-                 is_subject_asid aag x)"
-             in hoare_strengthen_post)
-    apply (simp add: page_bits_def)
-    apply (wp add: delete_objects_pspace_no_overlap hoare_vcg_ex_lift
-                   delete_objects_descendants_range_in delete_objects_invs_ex
-                   delete_objects_pas_refined
-              del: Untyped_AI.delete_objects_pspace_no_overlap
-          | simp add: page_bits_def)+
-   apply clarsimp
-   apply (rename_tac s idx)
-   apply (frule untyped_cap_aligned, simp add: invs_valid_objs)
-   apply (clarsimp simp: cte_wp_at_def aag_cap_auth_def ptr_range_def pas_refined_refl
-                         cap_links_asid_slot_def cap_links_irq_def
-                         obj_bits_api_def default_arch_object_def retype_addrs_def)
-   apply (rule conjI, force intro: descendants_range_caps_no_overlapI
-                             simp: cte_wp_at_def)
-   apply (rule conjI)
-    apply (cut_tac s=s and ptr="(parent_ptr, parent_idx)" in cap_refs_in_kernel_windowD)
-      apply ((fastforce simp add: caps_of_state_def cap_range_def)+)[3]
-   apply (rule conjI, force simp: field_simps)
-   apply (rule conjI, fastforce)
-   apply (fastforce dest: caps_of_state_valid
-                    simp: caps_of_state_def free_index_of_def
-                          max_free_index_def valid_cap_def)
-  apply (clarsimp simp: valid_aci_def authorised_asid_control_inv_def)
-  apply (rename_tac frame slot_ptr slot_idx parent_ptr parent_idx base)
-  apply (subgoal_tac "is_aligned frame pageBits")
-   apply (clarsimp simp: cte_wp_at_caps_of_state)
-   apply (rule conjI)
-    apply (drule untyped_slots_not_in_untyped_range)
-         apply (erule empty_descendants_range_in)
-        apply (simp add: cte_wp_at_caps_of_state)
-       apply simp
-      apply (rule refl)
-     apply (rule subset_refl)
-    apply (simp add: page_bits_def)
-   apply (clarsimp simp: ptr_range_def invs_psp_aligned invs_valid_objs
-                         descendants_range_def2 empty_descendants_range_in page_bits_def)
-   apply ((strengthen refl | simp)+)?
-   apply (rule conjI, fastforce)
-   apply (rule conjI, fastforce intro: empty_descendants_range_in)
-   apply (rule conjI)
-    apply (clarsimp simp: range_cover_def obj_bits_api_def default_arch_object_def)
-    apply (subst is_aligned_neg_mask_eq[THEN sym], assumption)
-    apply (simp add: and_mask_eq_iff_shiftr_0 pageBits_def mask_zero)
-   apply (clarsimp simp: aag_cap_auth_def pas_refined_refl)
-   apply (drule_tac x=frame in bspec)
-    apply (simp add: is_aligned_no_overflow)
-   apply (clarsimp simp: pas_refined_refl cap_links_asid_slot_def
-                         label_owns_asid_slot_def cap_links_irq_def)
-  apply (fastforce dest: cte_wp_at_valid_objs_valid_cap simp: valid_cap_def cap_aligned_def)
-  done
-
-lemma set_asid_pool_respects:
-  "\<lbrace>integrity aag X st and K (is_subject aag ptr)\<rbrace>
-     set_asid_pool ptr pool
-   \<lbrace>\<lambda>s. integrity aag X st\<rbrace>"
-  apply (simp add: set_asid_pool_def)
-  apply (wp get_object_wp set_object_integrity_autarch)
-  apply simp
-  done
-
-definition
-  authorised_asid_pool_inv :: "'a PAS \<Rightarrow> asid_pool_invocation \<Rightarrow> bool"
-where
- "authorised_asid_pool_inv aag api \<equiv> case api of
-     asid_pool_invocation.Assign asid pool_ptr ct_slot \<Rightarrow>
-       is_subject aag pool_ptr \<and> is_subject aag (fst ct_slot)
-          \<and> asid \<noteq> 0
-          \<and> (\<forall>asid'. asid_high_bits_of asid' = asid_high_bits_of asid \<and> asid' \<noteq> 0
-                     \<longrightarrow> is_subject_asid aag asid')"
-
-lemma perform_asid_pool_invocation_respects:
-  "\<lbrace>integrity aag X st and K (authorised_asid_pool_inv aag api)\<rbrace>
-     perform_asid_pool_invocation api
-   \<lbrace>\<lambda>s. integrity aag X st\<rbrace>"
-  apply (simp add: perform_asid_pool_invocation_def)
-  apply (rule hoare_pre)
-  apply (wp set_asid_pool_respects get_cap_wp set_cap_integrity_autarch
-       | wpc
-       | simp)+
-  apply (auto iff: authorised_asid_pool_inv_def)
-  done
-
-lemma is_subject_asid_into_loas:
-  "\<lbrakk> is_subject_asid aag asid; pas_refined aag s \<rbrakk> \<Longrightarrow> label_owns_asid_slot aag (pasSubject aag) asid"
-  unfolding label_owns_asid_slot_def
-  by (clarsimp simp: pas_refined_refl)
-
-lemma asid_pool_into_aag:
-  "\<lbrakk>kheap s p = Some (ArchObj (arch_kernel_obj.ASIDPool pool)); pool r = Some p'; pas_refined aag s \<rbrakk>
-  \<Longrightarrow> (pasObjectAbs aag p, Control, pasObjectAbs aag p') \<in> pasPolicy aag"
-  apply (rule pas_refined_mem [rotated], assumption)
-  apply (rule sta_vref)
-  apply (fastforce simp add: state_vrefs_def vs_refs_no_global_pts_def intro!: graph_ofI)
-  done
-
-lemma asid_pool_uniqueness:
-  "\<lbrakk> ([VSRef (ucast (asid_high_bits_of asid)) None] \<rhd> p) s;
-      arm_asid_table (arch_state s) (asid_high_bits_of asid') = Some p;
-       invs s; \<forall>pt. \<not> ko_at (ArchObj (PageTable pt)) p s \<rbrakk>
-      \<Longrightarrow> asid_high_bits_of asid' = asid_high_bits_of asid"
-  apply (drule valid_vs_lookupD[OF vs_lookup_pages_vs_lookupI], clarsimp)
-  apply (drule vs_lookup_atI, drule valid_vs_lookupD[OF vs_lookup_pages_vs_lookupI], clarsimp)
-  apply (clarsimp dest!: obj_ref_elemD)
-  apply (drule(1) unique_table_refsD[where cps="caps_of_state s", rotated])
+  apply (wpsimp wp: gets_the_wp get_wp put_wp mapM_x_wp'
+                    store_word_offs_integrity_autarch[where thread=thread]
+              simp: split_def zipWithM_x_mapM_x split_del: if_split)+
+     apply (clarsimp elim!: in_set_zipE split: if_split_asm)
+     apply (rule order_le_less_trans[where y=msg_max_length])
+      apply (fastforce simp add: le_eq_less_or_eq)
+     apply (simp add: msg_max_length_def msg_align_bits' word_size_bits_def)
     apply simp
-   apply (clarsimp simp: vs_cap_ref_def table_cap_ref_def up_ucast_inj_eq
-                  split: vmpage_size.splits option.splits cap.splits arch_cap.splits)+
-  done
-
-lemma perform_asid_pool_invocation_pas_refined [wp]:
-  "\<lbrace>pas_refined aag and invs and valid_apinv api and K (authorised_asid_pool_inv aag api)\<rbrace>
-     perform_asid_pool_invocation api
-   \<lbrace>\<lambda>_. pas_refined aag\<rbrace>"
-  apply (simp add: perform_asid_pool_invocation_def)
-  apply (rule hoare_pre)
-  apply (wp get_cap_auth_wp[where aag = aag] set_cap_pas_refined_not_transferable | wpc)+
-  apply (clarsimp simp: authorised_asid_pool_inv_def cap_links_asid_slot_def
-                        is_subject_asid_into_loas aag_cap_auth_def)
-  apply (clarsimp simp: cap_auth_conferred_def is_cap_simps is_page_cap_def auth_graph_map_mem
-                        pas_refined_all_auth_is_owns pas_refined_refl cli_no_irqs
-                        cte_wp_at_caps_of_state
-                 dest!: graph_ofD)
-  apply (clarsimp split: if_split_asm)
-   apply (clarsimp simp add: pas_refined_refl auth_graph_map_def2
-                             mask_asid_low_bits_ucast_ucast[symmetric]
-                             valid_apinv_def obj_at_def)
-   apply (drule(2) asid_pool_uniqueness)
-    apply (simp add: obj_at_def)
-   apply (case_tac "asid = 0"; simp add: pas_refined_refl)
-   apply (simp add: asid_low_high_bits[rotated, OF arg_cong[where f=ucast]])
-  apply (clarsimp simp: obj_at_def)
-  apply (frule (2) asid_pool_into_aag)
-  apply (drule kheap_eq_state_vrefsD)
-  apply (clarsimp simp: auth_graph_map_def2 pas_refined_refl)
-  apply (clarsimp simp: pas_refined_def vs_refs_no_global_pts_def)
-  apply (erule subsetD, erule state_asids_to_policy_aux.intros,
-         simp add: split_def, rule image_eqI[rotated], erule graph_ofI)
+    apply (wp set_object_integrity_autarch hoare_drop_imps hoare_vcg_all_lift)+
   apply simp
   done
-
-definition
-  authorised_page_directory_inv :: "'a PAS \<Rightarrow> page_directory_invocation \<Rightarrow> bool"
-where
-  "authorised_page_directory_inv aag pdi \<equiv> True"
-
-definition
-  authorised_arch_inv :: "'a PAS \<Rightarrow> arch_invocation \<Rightarrow> bool"
-where
- "authorised_arch_inv aag ai \<equiv> case ai of
-     InvokePageTable pti \<Rightarrow> authorised_page_table_inv aag pti
-   | InvokePageDirectory pdi \<Rightarrow> authorised_page_directory_inv aag pdi
-   | InvokePage pgi \<Rightarrow> authorised_page_inv aag pgi
-   | InvokeASIDControl aci \<Rightarrow> authorised_asid_control_inv aag aci
-   | InvokeASIDPool api \<Rightarrow> authorised_asid_pool_inv aag api"
-
-crunch respects [wp]: perform_page_directory_invocation "integrity aag X st"
-  (ignore: do_machine_op)
-
-lemma invoke_arch_respects:
-  "\<lbrace>integrity aag X st and K (authorised_arch_inv aag ai) and
-    pas_refined aag and invs and valid_arch_inv ai and is_subject aag \<circ> cur_thread\<rbrace>
-     arch_perform_invocation ai
-   \<lbrace>\<lambda>s. integrity aag X st\<rbrace>"
-  apply (simp add: arch_perform_invocation_def)
-  apply (rule hoare_pre)
-  apply (wp perform_page_table_invocation_respects perform_page_invocation_respects
-           perform_asid_control_invocation_respects perform_asid_pool_invocation_respects
-       | wpc)+
-  apply (auto simp: authorised_arch_inv_def valid_arch_inv_def)
-  done
-
-crunch pas_refined [wp]: perform_page_directory_invocation "pas_refined aag"
-
-lemma invoke_arch_pas_refined:
-  "\<lbrace>pas_refined aag and pas_cur_domain aag and invs and ct_active and valid_arch_inv ai and K (authorised_arch_inv aag ai)\<rbrace>
-     arch_perform_invocation ai
-   \<lbrace>\<lambda>s. pas_refined aag\<rbrace>"
-  apply (simp add: arch_perform_invocation_def valid_arch_inv_def)
-  apply (rule hoare_pre)
-  apply (wp | wpc)+
-  apply (fastforce simp add: authorised_arch_inv_def)
-  done
-
-lemma create_mapping_entries_authorised_slots [wp]:
-  "\<lbrace>\<exists>\<rhd> pd and invs and pas_refined aag
-    and K (is_subject aag pd
-           \<and> is_aligned pd pd_bits
-           \<and> vmsz_aligned vptr vmpage_size
-           \<and> vptr < kernel_base
-           \<and> (\<forall>a\<in>vspace_cap_rights_to_auth rights.
-                  \<forall>p\<in>ptr_range (ptrFromPAddr base) (pageBitsForSize vmpage_size).
-                      aag_has_auth_to aag a p))\<rbrace>
-    create_mapping_entries base vptr vmpage_size rights attrib pd
-  \<lbrace>\<lambda>rv s. authorised_slots aag rv\<rbrace>, -"
-  unfolding authorised_slots_def
-  apply (rule hoare_gen_asmE)
-  apply (cases vmpage_size)
-     apply (wp lookup_pt_slot_authorised
-                 | simp add: pte_ref_simps | fold validE_R_def)+
-     apply (auto simp: pd_bits_def pageBits_def)[1]
-    apply (wp lookup_pt_slot_authorised2
-          | simp add: pte_ref_simps largePagePTE_offsets_def
-          | fold validE_R_def)+
-    apply (auto simp: pd_bits_def pageBits_def vmsz_aligned_def)[1]
-   apply (wp | simp)+
-   apply (auto simp: pde_ref2_def lookup_pd_slot_pd)[1]
-  apply (wp | simp add: superSectionPDE_offsets_def)+
-  apply (auto simp: pde_ref2_def vmsz_aligned_def lookup_pd_slot_add_eq)
-  done
-
-lemma x_t2n_sub_1_neg_mask:
-  "\<lbrakk> is_aligned x n; n \<le> m \<rbrakk>
-     \<Longrightarrow> x + 2 ^ n - 1 && ~~ mask m = x && ~~ mask m"
-  apply (erule is_aligned_get_word_bits)
-   apply (rule trans, rule mask_lower_twice[symmetric], assumption)
-   apply (subst add_diff_eq[symmetric], subst is_aligned_add_helper, assumption)
-    apply simp+
-  apply (simp add: mask_def power_overflow)
-  done
-
-lemma pageBitsForSize_le_t28:
-  "pageBitsForSize sz \<le> 28"
-  by (cases sz, simp_all)
-
-lemma pageBitsForSize_le_t29:
-  "pageBitsForSize sz \<le> 29"
-  by (cases sz, simp_all)
-
-lemmas vmsz_aligned_t2n_neg_mask
-    = x_t2n_sub_1_neg_mask[OF _ pageBitsForSize_le_t29, folded vmsz_aligned_def]
-
-lemma decode_arch_invocation_authorised:
-  "\<lbrace>invs and pas_refined aag
-        and cte_wp_at ((=) (cap.ArchObjectCap cap)) slot
-        and (\<lambda>s. \<forall>(cap, slot) \<in> set excaps. cte_wp_at ((=) cap) slot s)
-        and K (\<forall>(cap, slot) \<in> {(cap.ArchObjectCap cap, slot)} \<union> set excaps.
-                      aag_cap_auth aag (pasObjectAbs aag (fst slot)) cap \<and> is_subject aag (fst slot)
-                   \<and> (\<forall>v \<in> cap_asid' cap. is_subject_asid aag v))\<rbrace>
-     arch_decode_invocation label msg x_slot slot cap excaps
-   \<lbrace>\<lambda>rv s. authorised_arch_inv aag rv\<rbrace>,-"
-  unfolding arch_decode_invocation_def authorised_arch_inv_def aag_cap_auth_def
-  apply (rule hoare_pre)
-   apply (simp add: split_def Let_def
-     cong: cap.case_cong arch_cap.case_cong if_cong option.case_cong split del: if_split)
-
-   apply (wp select_wp whenE_throwError_wp check_vp_wpR
-             find_pd_for_asid_authority2
-           | wpc
-           | simp add: authorised_asid_control_inv_def authorised_page_inv_def
-                       authorised_page_directory_inv_def
-                  del: hoare_True_E_R
-                  split del: if_split)+
-  apply (clarsimp simp: authorised_asid_pool_inv_def authorised_page_table_inv_def
-                        neq_Nil_conv invs_psp_aligned invs_vspace_objs cli_no_irqs)
-  apply (drule cte_wp_valid_cap, clarsimp+)
-  apply (cases cap; simp)
-      \<comment> \<open>asid pool\<close>
-     apply (find_goal \<open>match premises in "cap = ASIDPoolCap _ _" \<Rightarrow> succeed\<close>)
-     subgoal for s obj_ref asid
-       by (clarsimp simp: cap_auth_conferred_def is_page_cap_def
-                          pas_refined_all_auth_is_owns asid_high_bits_of_add_ucast
-                          valid_cap_simps)
-     \<comment> \<open>ControlCap\<close>
-    apply (find_goal \<open>match premises in "cap = ASIDControlCap" \<Rightarrow> succeed\<close>)
-    subgoal
-      apply (clarsimp simp: neq_Nil_conv split_def valid_cap_simps)
-      apply (cases excaps, solves simp)
-      apply (clarsimp simp: neq_Nil_conv aag_has_auth_to_Control_eq_owns)
-      apply (drule cte_wp_at_valid_objs_valid_cap, clarsimp)
-      apply (clarsimp simp: valid_cap_def cap_aligned_def)
-      apply (clarsimp simp: is_cap_simps cap_auth_conferred_def
-                            pas_refined_all_auth_is_owns aag_cap_auth_def)
-      done
-   \<comment> \<open>PageCap\<close>
-   apply (find_goal \<open>match premises in "cap = PageCap _ _ _ _ _" \<Rightarrow> succeed\<close>)
-   subgoal for s is_dev obj_ref cap_rights vmpage_size mapping
-     apply (clarsimp simp: valid_cap_simps cli_no_irqs)
-     apply (cases "invocation_type label"; (solves \<open>simp\<close>)?)
-     apply (find_goal \<open>match premises in "_ = ArchInvocationLabel _" \<Rightarrow> succeed\<close>)
-     apply (rename_tac archlabel)
-     apply (case_tac archlabel; (solves \<open>simp\<close>)?)
-       \<comment> \<open>Map\<close>
-      apply (find_goal \<open>match premises in "_ = ARMPageMap" \<Rightarrow> succeed\<close>)
-      subgoal
-       apply (clarsimp simp: cap_auth_conferred_def is_cap_simps is_page_cap_def
-                             pas_refined_all_auth_is_owns)
-       apply (rule conjI)
-        apply (clarsimp simp: cap_auth_conferred_def is_page_cap_def pas_refined_all_auth_is_owns
-                              aag_cap_auth_def cli_no_irqs cap_links_asid_slot_def)
-        apply (simp only: linorder_not_le kernel_base_less_observation
-                          vmsz_aligned_t2n_neg_mask simp_thms)
-        apply (clarsimp simp: cap_auth_conferred_def vspace_cap_rights_to_auth_def
-                              mask_vm_rights_def validate_vm_rights_def vm_read_only_def
-                              vm_kernel_only_def)
-       apply (clarsimp simp: cap_auth_conferred_def is_cap_simps is_page_cap_def
-                             pas_refined_all_auth_is_owns)
-       apply (rule conjI)
-        apply (clarsimp simp: cap_auth_conferred_def is_page_cap_def pas_refined_all_auth_is_owns
-                              aag_cap_auth_def cli_no_irqs cap_links_asid_slot_def)
-       apply (clarsimp simp: cap_auth_conferred_def vspace_cap_rights_to_auth_def
-                             mask_vm_rights_def validate_vm_rights_def vm_read_only_def
-                             vm_kernel_only_def)
-       done
-     \<comment> \<open>Unmap\<close>
-     subgoal by (simp add: aag_cap_auth_def cli_no_irqs)
-     done
-  \<comment> \<open>PageTableCap\<close>
-  apply (find_goal \<open>match premises in "cap = PageTableCap _ _" \<Rightarrow> succeed\<close>)
-  subgoal for s word option
-    apply (cases "invocation_type label"; (solves \<open>simp\<close>)?)
-    apply (find_goal \<open>match premises in "_ = ArchInvocationLabel _" \<Rightarrow> succeed\<close>)
-    apply (rename_tac archlabel)
-    apply (case_tac archlabel; (solves \<open>simp\<close>)?)
-     \<comment> \<open>PTMap\<close>
-     apply (find_goal \<open>match premises in "_ = ARMPageTableMap" \<Rightarrow> succeed\<close>)
-     apply (clarsimp simp: aag_cap_auth_def cli_no_irqs cap_links_asid_slot_def
-                           cap_auth_conferred_def is_page_cap_def
-                           pde_ref2_def pas_refined_all_auth_is_owns pas_refined_refl
-                           pd_shifting[folded pd_bits_14])
-    \<comment> \<open>Unmap\<close>
-    apply (find_goal \<open>match premises in "_ = ARMPageTableUnmap" \<Rightarrow> succeed\<close>)
-    subgoal
-      apply (clarsimp simp: aag_cap_auth_def cli_no_irqs cap_links_asid_slot_def
-                            cap_auth_conferred_def is_page_cap_def
-                            pde_ref2_def pas_refined_all_auth_is_owns pas_refined_refl)
-      apply (subgoal_tac "x && ~~ mask pt_bits = word")
-       apply simp
-      apply (clarsimp simp: valid_cap_simps cap_aligned_def split: if_split_asm)
-      apply (subst (asm) upto_enum_step_subtract)
-      apply (subgoal_tac "is_aligned word pt_bits")
-       apply (simp add: is_aligned_no_overflow)
-      apply (simp add: pt_bits_def pageBits_def)
-      apply simp
-      apply (subst (asm) upto_enum_step_red [where us = 2, simplified])
-      apply (simp add: pt_bits_def pageBits_def word_bits_conv)
-      apply (simp add: pt_bits_def pageBits_def word_bits_conv)
-      apply clarsimp
-      apply (subst is_aligned_add_helper)
-      apply (simp add: pt_bits_def pageBits_def)
-      apply (erule word_less_power_trans_ofnat [where k = 2, simplified])
-        apply (simp add: pt_bits_def pageBits_def)
-       apply (simp add: pt_bits_def pageBits_def word_bits_conv)
-      apply simp
-      done
-    done
-  done
-
-crunch pas_refined[wp]: invalidate_asid_entry "pas_refined aag"
-  (wp: crunch_wps simp: crunch_simps)
-
-crunch pas_refined[wp]: flush_space "pas_refined aag"
-  (wp: crunch_wps simp: crunch_simps)
-
-lemma delete_asid_pas_refined[wp]:
-  "\<lbrace>pas_refined aag\<rbrace> delete_asid asid pd \<lbrace>\<lambda>rv. pas_refined aag\<rbrace>"
-  apply (simp add: delete_asid_def)
-  apply (wp | wpc)+
-  apply (clarsimp simp add: split_def Ball_def obj_at_def)
-  apply (rule conjI)
-   apply (clarsimp dest!: auth_graph_map_memD graph_ofD)
-   apply (erule pas_refined_mem[OF sta_vref, rotated])
-   apply (fastforce simp: state_vrefs_def vs_refs_no_global_pts_def
-                         image_def graph_of_def split: if_split_asm)
-  apply (clarsimp simp: pas_refined_def dest!: graph_ofD)
-  apply (erule subsetD, erule state_asids_to_policy_aux.intros)
-  apply (fastforce simp: state_vrefs_def vs_refs_no_global_pts_def
-                        graph_of_def image_def split: if_split_asm)
-  done
-
-lemma delete_asid_pool_pas_refined [wp]:
-  "\<lbrace>pas_refined aag\<rbrace> delete_asid_pool param_a param_b \<lbrace>\<lambda>_. pas_refined aag\<rbrace>"
-  unfolding delete_asid_pool_def
-  apply (wp | wpc | simp)+
-  apply (rule_tac Q = "\<lambda>_ s. pas_refined aag s \<and> asid_table = arm_asid_table (arch_state s)" in hoare_post_imp)
-  apply clarsimp
-  apply (erule pas_refined_clear_asid)
-  apply (wp mapM_wp' | simp)+
-  done
-
-crunch respects[wp]: invalidate_asid_entry "integrity aag X st"
-
-crunch respects[wp]: flush_space "integrity aag X st"
-  (ignore: do_machine_op simp: invalidateLocalTLB_ASID_def cleanCaches_PoU_def dsb_def clean_D_PoU_def invalidate_I_PoU_def do_machine_op_bind)
-
-lemma delete_asid_pool_respects[wp]:
-  "\<lbrace> integrity aag X st and K (\<forall>asid'.
-            asid' \<noteq> 0 \<and> asid_high_bits_of asid' = asid_high_bits_of x \<longrightarrow>
-            is_subject_asid aag asid')\<rbrace>
-   delete_asid_pool x y
-   \<lbrace> \<lambda>_. integrity aag X st \<rbrace>"
-  unfolding delete_asid_pool_def
-  apply simp
-  apply (wp mapM_wp[OF _ subset_refl] | simp)+
-  done
-
-
-lemma pas_refined_asid_mem:
-  "\<lbrakk> v \<in> state_asids_to_policy aag s; pas_refined aag s \<rbrakk>
-         \<Longrightarrow> v \<in> pasPolicy aag"
-  by (auto simp add: pas_refined_def)
-
-
-lemma set_asid_pool_respects_clear:
-  "\<lbrace>(\<lambda>s. \<forall>pool'. ko_at (ArchObj (arch_kernel_obj.ASIDPool pool')) ptr s
-              \<longrightarrow> asid_pool_integrity {pasSubject aag} aag pool' pool)
-            and integrity aag X st\<rbrace>
-     set_asid_pool ptr pool \<lbrace>\<lambda>rv. integrity aag X st\<rbrace>"
-  apply (simp add: set_asid_pool_def)
-  apply (wpsimp wp: set_object_wp_strong
-              simp: obj_at_def a_type_def
-             split: Structures_A.kernel_object.split_asm arch_kernel_obj.split_asm if_splits)
-  apply (erule integrity_trans)
-  apply (clarsimp simp: integrity_def)
-  apply (rule tro_asidpool_clear; simp add: asid_pool_integrity_def)
-  done
-
-lemma delete_asid_respects:
-  "\<lbrace>integrity aag X st and pas_refined aag and invs and K (is_subject aag pd)\<rbrace>
-     delete_asid asid pd
-   \<lbrace>\<lambda>rv. integrity aag X st\<rbrace>"
-  by (wpsimp wp: set_asid_pool_respects_clear hoare_vcg_all_lift
-           simp: obj_at_def pas_refined_refl delete_asid_def asid_pool_integrity_def)
 
 end
 
