proof/access-control/ARM/ArchArch_AC.thy
@@ -1,0 +1,1002 @@
+(*
+ * Copyright 2020, Data61, CSIRO (ABN 41 687 119 230)
+ *
+ * SPDX-License-Identifier: GPL-2.0-only
+ *)
+
+theory ArchArch_AC
+imports Arch_AC
+begin
+
+text\<open>
+
+Arch-specific access control.
+
+\<close>
+
+context Arch begin global_naming ARM_A
+
+named_theorems Arch_AC_assms
+
+lemma set_mrs_state_vrefs[Arch_AC_assms, wp]:
+  "set_mrs thread buf msgs \<lbrace>\<lambda>s. P (state_vrefs s)\<rbrace>"
+  apply (simp add: set_mrs_def split_def set_object_def get_object_def split del: if_split)
+  apply (wpsimp wp: gets_the_wp get_wp put_wp mapM_x_wp'
+              simp: zipWithM_x_mapM_x split_def store_word_offs_def
+         split_del: if_split)
+  apply (auto simp: obj_at_def state_vrefs_def get_tcb_ko_at
+             elim!: rsubst[where P=P, OF _ ext]
+             split: if_split_asm simp: vs_refs_no_global_pts_def)
+  done
+
+lemma mul_add_word_size_lt_msg_align_bits_ofnat[Arch_AC_assms]:
+  "\<lbrakk> p < 2 ^ (msg_align_bits - word_size_bits); k < 4 \<rbrakk>
+     \<Longrightarrow> of_nat p * of_nat word_size + k < (2 :: obj_ref) ^ msg_align_bits"
+  apply (rule is_aligned_add_less_t2n[where n=word_size_bits])
+     apply (simp_all add: msg_align_bits' word_size_word_size_bits is_aligned_mult_triv2)
+   apply (simp_all add: word_size_word_size_bits word_size_bits_def)
+  apply (erule word_less_power_trans_ofnat[where k=2 and m=9, simplified], simp)
+  done
+
+end
+
+
+global_interpretation Arch_AC_1?: Arch_AC_1
+proof goal_cases
+  interpret Arch .
+  case 1 show ?case
+    by (unfold_locales; fact Arch_AC_assms)
+qed
+
+
+context Arch begin global_naming ARM_A
+
+lemma store_pte_respects:
+  "\<lbrace>integrity aag X st and K (is_subject aag (p && ~~ mask pt_bits))\<rbrace>
+   store_pte p pte
+   \<lbrace>\<lambda>_. integrity aag X st\<rbrace>"
+  apply (simp add: store_pte_def set_pt_def)
+  apply (wp get_object_wp set_object_integrity_autarch)
+  apply simp
+  done
+
+lemma integrity_arch_state [iff]:
+  "arm_asid_table v = arm_asid_table (arch_state s)
+   \<Longrightarrow> integrity aag X st (s\<lparr>arch_state := v\<rparr>) = integrity aag X st s"
+  unfolding integrity_def by simp
+
+lemma integrity_arm_asid_map[iff]:
+  "integrity aag X st (s\<lparr>arch_state := ((arch_state s)\<lparr>arm_asid_map := v\<rparr>)\<rparr>) =
+   integrity aag X st s"
+  unfolding integrity_def by simp
+
+lemma integrity_arm_hwasid_table[iff]:
+  "integrity aag X st (s\<lparr>arch_state := ((arch_state s)\<lparr>arm_hwasid_table := v\<rparr>)\<rparr>) =
+   integrity aag X st s"
+  unfolding integrity_def by simp
+
+lemma integrity_arm_next_asid[iff]:
+  "integrity aag X st (s\<lparr>arch_state := ((arch_state s)\<lparr>arm_next_asid := v\<rparr>)\<rparr>) =
+   integrity aag X st s"
+  unfolding integrity_def by simp
+
+crunch respects[wp]: arm_context_switch "integrity X aag st"
+  (simp: dmo_bind_valid dsb_def isb_def writeTTBR0_def invalidateLocalTLB_ASID_def
+         setHardwareASID_def set_current_pd_def ignore: do_machine_op)
+
+crunch respects[wp]: set_vm_root "integrity X aag st"
+  (simp: set_current_pd_def isb_def dsb_def writeTTBR0_def dmo_bind_valid crunch_simps
+     wp: crunch_wps ignore: do_machine_op)
+
+crunch respects[wp]: set_vm_root_for_flush "integrity X aag st"
+  (wp: crunch_wps simp: set_current_pd_def crunch_simps ignore: do_machine_op)
+
+crunch respects[wp]: flush_table "integrity X aag st"
+  (wp: crunch_wps simp: invalidateLocalTLB_ASID_def crunch_simps ignore: do_machine_op)
+
+crunch respects[wp]: page_table_mapped "integrity X aag st"
+
+lemma kheap_eq_state_vrefsD:
+  "kheap s p = Some ko \<Longrightarrow> state_vrefs s p = vs_refs_no_global_pts ko"
+  by (simp add: state_vrefs_def)
+
+lemma kheap_eq_state_vrefs_pas_refinedD:
+  "\<lbrakk> kheap s p = Some ko; (p', r, t, a) \<in> vs_refs_no_global_pts ko; pas_refined aag s \<rbrakk>
+     \<Longrightarrow> abs_has_auth_to aag a p p'"
+  apply (drule kheap_eq_state_vrefsD)
+  apply (erule pas_refined_mem[OF sta_vref, rotated])
+  apply simp
+  done
+
+lemma find_pd_for_asid_authority1:
+  "\<lbrace>pas_refined aag\<rbrace>
+   find_pd_for_asid asid
+   \<lbrace>\<lambda>pd _. (pasASIDAbs aag asid, Control, pasObjectAbs aag pd) \<in> pasPolicy aag\<rbrace>,-"
+  apply (rule hoare_pre)
+   apply (simp add: find_pd_for_asid_def)
+   apply (wp | wpc)+
+  apply (clarsimp simp: obj_at_def pas_refined_def)
+  apply (erule subsetD, erule sata_asid_lookup)
+  apply (simp add: state_vrefs_def vs_refs_no_global_pts_def image_def)
+  apply (rule rev_bexI, erule graph_ofI)
+  apply (simp add: mask_asid_low_bits_ucast_ucast)
+  done
+
+lemma find_pd_for_asid_authority2:
+  "\<lbrace>\<lambda>s. \<forall>pd. (\<forall>aag. pas_refined aag s
+                    \<longrightarrow> (pasASIDAbs aag asid, Control, pasObjectAbs aag pd) \<in> pasPolicy aag) \<and>
+             (pspace_aligned s \<and> valid_vspace_objs s \<longrightarrow> is_aligned pd pd_bits) \<and>
+             (\<exists>\<rhd> pd) s
+             \<longrightarrow> Q pd s\<rbrace>
+   find_pd_for_asid asid
+   \<lbrace>Q\<rbrace>, -" (is "\<lbrace>?P\<rbrace> ?f \<lbrace>Q\<rbrace>,-")
+  apply (clarsimp simp: validE_R_def validE_def valid_def imp_conjL[symmetric])
+  apply (frule in_inv_by_hoareD[OF find_pd_for_asid_inv], clarsimp)
+  apply (drule spec, erule mp)
+  apply (simp add: use_validE_R[OF _ find_pd_for_asid_authority1]
+                   use_validE_R[OF _ find_pd_for_asid_aligned_pd_bits]
+                   use_validE_R[OF _ find_pd_for_asid_lookup])
+  done
+
+lemma find_pd_for_asid_pd_slot_authorised [wp]:
+  "\<lbrace>pas_refined aag and K (is_subject_asid aag asid) and pspace_aligned and valid_vspace_objs\<rbrace>
+   find_pd_for_asid asid
+   \<lbrace>\<lambda>rv _. is_subject aag (lookup_pd_slot rv vptr && ~~ mask pd_bits)\<rbrace>, -"
+  apply (wp find_pd_for_asid_authority2)
+  apply (clarsimp simp: lookup_pd_slot_pd)
+  apply (fastforce dest: pas_refined_Control)
+  done
+
+lemma unmap_page_table_respects:
+  "\<lbrace>integrity aag X st and pas_refined aag and invs
+                       and K (is_subject_asid aag asid \<and> vaddr < kernel_base)\<rbrace>
+   unmap_page_table asid vaddr pt
+   \<lbrace>\<lambda>_. integrity aag X st\<rbrace>"
+  apply (rule hoare_gen_asm)
+  apply (simp add: unmap_page_table_def page_table_mapped_def )
+  apply (rule hoare_pre)
+   apply (wpsimp wp: store_pde_respects page_table_mapped_wp_weak get_pde_wp hoare_vcg_all_lift_R
+               simp: cleanByVA_PoU_def
+          | wp (once) hoare_drop_imps)+
+  apply auto
+  done
+
+definition authorised_page_table_inv :: "'a PAS \<Rightarrow> page_table_invocation \<Rightarrow> bool" where
+  "authorised_page_table_inv aag pti \<equiv>
+   case pti of PageTableMap cap cslot_ptr pde obj_ref \<Rightarrow>
+                 is_subject aag (fst cslot_ptr) \<and> is_subject aag (obj_ref && ~~ mask pd_bits) \<and>
+                 (case_option True (is_subject aag o fst) (pde_ref2 pde)) \<and>
+                 pas_cap_cur_auth aag cap
+             | PageTableUnmap cap cslot_ptr \<Rightarrow>
+                 is_subject aag (fst cslot_ptr) \<and> aag_cap_auth aag (pasSubject aag) cap  \<and>
+                 (\<forall>p asid vspace_ref. cap = ArchObjectCap (PageTableCap p (Some (asid, vspace_ref)))
+                                      \<longrightarrow> is_subject_asid aag asid \<and>
+                                          (\<forall>x \<in> set [p , p + 4 .e. p + 2 ^ pt_bits - 1].
+                                                   is_subject aag (x && ~~ mask pt_bits)))"
+
+lemma perform_page_table_invocation_respects:
+  "\<lbrace>integrity aag X st and pas_refined aag and invs and valid_pti page_table_invocation
+                       and K (authorised_page_table_inv aag page_table_invocation)\<rbrace>
+   perform_page_table_invocation page_table_invocation
+   \<lbrace>\<lambda>_. integrity aag X st\<rbrace>"
+  apply (rule hoare_gen_asm)
+  apply (simp add: perform_page_table_invocation_def
+             cong: page_table_invocation.case_cong option.case_cong prod.case_cong
+                   cap.case_cong arch_cap.case_cong)
+  apply (wpsimp wp: store_pde_respects set_cap_integrity_autarch
+                    store_pte_respects unmap_page_table_respects mapM_wp'
+              simp: mapM_x_mapM authorised_page_table_inv_def cleanByVA_PoU_def)
+  apply (auto simp: valid_pti_def valid_cap_simps)
+  done
+
+crunch arm_asid_table_inv [wp]: unmap_page_table "\<lambda>s. P (arm_asid_table (arch_state s))"
+  (wp: crunch_wps simp: crunch_simps)
+
+lemma clas_update_map_data_strg:
+  "(is_pg_cap cap \<or> is_pt_cap cap)
+   \<longrightarrow> cap_links_asid_slot aag p (ArchObjectCap (update_map_data (the_arch_cap cap) None))"
+  unfolding cap_links_asid_slot_def
+  by (fastforce simp: is_cap_simps update_map_data_def)
+
+lemmas pte_ref_simps = pte_ref_def[split_simps pte.split]
+
+lemmas store_pde_pas_refined_simple =
+  store_pde_pas_refined[where pde=InvalidPDE, simplified pde_ref_simps, simplified]
+
+crunch pas_refined[wp]: unmap_page_table "pas_refined aag"
+  (wp: crunch_wps store_pde_pas_refined_simple simp: crunch_simps pde_ref_simps)
+
+lemma pde_ref_pde_ref2:
+  "\<lbrakk> pde_ref x = Some v; pde_ref2 x = Some v' \<rbrakk>
+     \<Longrightarrow> v' = (v, 0, {Control})"
+  unfolding pde_ref_def pde_ref2_def
+  by (cases x, simp_all)
+
+lemma mask_PTCap_eq:
+  "(ArchObjectCap (PageTableCap a b) = mask_cap R cap) = (cap = ArchObjectCap (PageTableCap a b))"
+  by (auto simp: mask_cap_def cap_rights_update_def acap_rights_update_def
+          split: arch_cap.splits cap.splits bool.splits)
+
+(* FIXME MOVE *)
+crunch cdt[wp]: unmap_page_table "\<lambda>s. P (cdt s)"
+  (simp: crunch_simps wp: crunch_wps)
+
+lemma is_transferable_is_arch_update:
+  "is_arch_update cap cap' \<Longrightarrow> is_transferable (Some cap) = is_transferable (Some cap')"
+  using is_transferable.simps is_arch_cap_def is_arch_update_def cap_master_cap_def
+  by (simp split: cap.splits arch_cap.splits)
+
+lemma perform_page_table_invocation_pas_refined [wp]:
+  "\<lbrace>pas_refined aag and valid_pti iv and K (authorised_page_table_inv aag iv)\<rbrace>
+   perform_page_table_invocation iv
+   \<lbrace>\<lambda>_. pas_refined aag\<rbrace>"
+  apply (rule hoare_gen_asm)
+  apply (simp add: perform_page_table_invocation_def
+             cong: page_table_invocation.case_cong option.case_cong prod.case_cong
+                   cap.case_cong arch_cap.case_cong)
+  apply (rule hoare_pre)
+  apply (wp get_cap_wp mapM_wp' store_pte_cte_wp_at do_machine_op_cte_wp_at
+            hoare_vcg_all_lift set_cap_pas_refined_not_transferable
+         | (wp hoare_vcg_imp_lift, unfold disj_not1)
+         | simp add: mapM_x_mapM authorised_page_table_inv_def imp_conjR pte_ref_simps
+         | wpc | wps| blast)+
+  apply (cases iv)
+   apply (fastforce simp: cte_wp_at_caps_of_state Option.is_none_def
+                          is_transferable_is_arch_update[symmetric]
+                          valid_pti_def is_cap_simps pas_refined_refl auth_graph_map_def2
+                    dest: pde_ref_pde_ref2)
+  apply (rename_tac s pt_cap page_cslot)
+  apply (case_tac page_cslot)
+  apply (rename_tac page_ptr page_slot)
+  apply (case_tac "\<exists>pt_ptr mapping. pt_cap = ArchObjectCap (PageTableCap pt_ptr mapping)")
+   prefer 2
+   apply fastforce
+  apply (elim exE)
+  apply clarsimp
+  apply (rename_tac page_cap)
+  apply (subgoal_tac
+            "cte_wp_at ((=) page_cap) (page_ptr, page_slot) s \<longrightarrow>
+             cte_wp_at (\<lambda>c. \<not> is_transferable (Some c)) (page_ptr, page_slot) s \<and>
+             pas_cap_cur_auth aag (ArchObjectCap (update_map_data (the_arch_cap page_cap) None))")
+   apply simp
+  apply (clarsimp simp: cte_wp_at_caps_of_state)
+  apply (frule (1) cap_cur_auth_caps_of_state)
+   apply simp
+  apply (clarsimp simp: valid_pti_def cte_wp_at_caps_of_state mask_PTCap_eq)
+  apply (clarsimp simp: cap_auth_conferred_def arch_cap_auth_conferred_def update_map_data_def
+                        is_page_cap_def cap_links_asid_slot_def cap_links_irq_def aag_cap_auth_def)
+  done
+
+definition authorised_slots :: "'a PAS \<Rightarrow> pte \<times> obj_ref list + pde \<times> obj_ref list \<Rightarrow> bool" where
+ "authorised_slots aag m \<equiv> case m of
+    Inl (pte, slots) \<Rightarrow>
+      (\<forall>x. pte_ref pte = Some x
+           \<longrightarrow> (\<forall>a \<in> snd (snd x). \<forall>p \<in> ptr_range (fst x) (fst (snd x)). aag_has_auth_to aag a p)) \<and>
+      (\<forall>x \<in> set slots. is_subject aag (x && ~~ mask pt_bits))
+  | Inr (pde, slots) \<Rightarrow>
+      (\<forall>x. pde_ref2 pde = Some x
+           \<longrightarrow> (\<forall>a \<in> snd (snd x). \<forall>p \<in> ptr_range (fst x) (fst (snd x)). aag_has_auth_to aag a p)) \<and>
+      (\<forall>x \<in> set slots. is_subject aag (x && ~~ mask pd_bits))"
+
+definition authorised_page_inv :: "'a PAS \<Rightarrow> page_invocation \<Rightarrow> bool" where
+  "authorised_page_inv aag pgi \<equiv> case pgi of
+     PageMap asid cap ptr slots \<Rightarrow>
+       pas_cap_cur_auth aag cap \<and> is_subject aag (fst ptr) \<and> authorised_slots aag slots
+   | PageUnmap cap ptr \<Rightarrow> pas_cap_cur_auth aag (ArchObjectCap cap) \<and> is_subject aag (fst ptr)
+   | PageFlush typ start end pstart pd asid \<Rightarrow> True
+   | PageGetAddr ptr \<Rightarrow> True"
+
+crunch respects[wp]: lookup_pt_slot "integrity X aag st"
+
+lemma vs_refs_no_global_pts_pdI:
+  "\<lbrakk> pd (ucast r) = PageTablePDE x a b; (ucast r :: 12 word) < ucast (kernel_base >> 20) \<rbrakk>
+     \<Longrightarrow> (ptrFromPAddr x, r && mask 12, APageDirectory, Control) \<in>
+           vs_refs_no_global_pts (ArchObj (PageDirectory pd))"
+  apply (clarsimp simp: vs_refs_no_global_pts_def)
+  apply (drule_tac f=pde_ref2 in arg_cong, simp add: pde_ref_simps o_def)
+  apply (rule rev_bexI, rule DiffI, erule graph_ofI)
+   apply simp
+  apply (clarsimp simp: ucast_ucast_mask)
+  done
+
+lemma lookup_pt_slot_authorised:
+  "\<lbrace>\<exists>\<rhd> pd and valid_vspace_objs and pspace_aligned and pas_refined aag
+          and K (is_subject aag pd) and K (is_aligned pd 14 \<and> vptr < kernel_base)\<rbrace>
+   lookup_pt_slot pd vptr
+   \<lbrace>\<lambda>rv _. is_subject aag (rv && ~~ mask pt_bits)\<rbrace>, -"
+  apply (simp add: lookup_pt_slot_def)
+  apply (wp get_pde_wp | wpc)+
+  apply (subgoal_tac "is_aligned pd pd_bits")
+   apply (clarsimp simp: lookup_pd_slot_pd)
+   apply (drule(2) valid_vspace_objsD)
+   apply (clarsimp simp: obj_at_def)
+   apply (drule kheap_eq_state_vrefs_pas_refinedD)
+     apply (erule vs_refs_no_global_pts_pdI)
+     apply (drule(1) less_kernel_base_mapping_slots)
+     apply (simp add: kernel_mapping_slots_def)
+    apply assumption
+   apply (simp add: aag_has_Control_iff_owns)
+   apply (drule_tac f="\<lambda>pde. valid_pde pde s" in arg_cong, simp)
+   apply (clarsimp simp: obj_at_def less_kernel_base_mapping_slots)
+   apply (erule pspace_alignedE, erule domI)
+   apply (simp add: pt_bits_def pageBits_def)
+   apply (subst is_aligned_add_helper, assumption)
+    apply (rule shiftl_less_t2n)
+     apply (rule order_le_less_trans, rule word_and_le1, simp)
+    apply simp
+   apply simp
+  apply (simp add: pd_bits_def pageBits_def)
+  done
+
+lemma is_aligned_6_masks:
+  "\<lbrakk> is_aligned (p :: obj_ref) 6; bits = pt_bits \<or> bits = pd_bits \<rbrakk>
+     \<Longrightarrow> \<forall>x \<in> set [0, 4 .e. 0x3C]. x + p && ~~ mask bits = p && ~~ mask bits"
+  apply clarsimp
+  apply (drule subsetD[OF upto_enum_step_subset])
+  apply (subst mask_lower_twice[symmetric, where n=6])
+   apply (auto simp add: pt_bits_def pageBits_def pd_bits_def)[1]
+  apply (subst add.commute, subst is_aligned_add_helper, assumption)
+   apply (simp add: order_le_less_trans)
+  apply simp
+  done
+
+lemma lookup_pt_slot_authorised2:
+  "\<lbrace>\<exists>\<rhd> pd and K (is_subject aag pd) and
+    K (is_aligned pd 14 \<and> is_aligned vptr 16 \<and> vptr < kernel_base) and
+    valid_vspace_objs and valid_arch_state and equal_kernel_mappings and
+    valid_global_objs and pspace_aligned and pas_refined aag\<rbrace>
+   lookup_pt_slot pd vptr
+   \<lbrace>\<lambda>rv _. \<forall>x\<in>set [0 , 4 .e. 0x3C]. is_subject aag (x + rv && ~~ mask pt_bits)\<rbrace>, -"
+  apply (clarsimp simp: validE_R_def valid_def validE_def
+                 split: sum.split)
+  apply (frule use_validE_R[OF _ lookup_pt_slot_authorised])
+   apply fastforce
+  apply (frule use_validE_R[OF _ lookup_pt_slot_is_aligned_6])
+   apply (fastforce simp add: vmsz_aligned_def pd_bits_def pageBits_def)
+  apply (simp add: is_aligned_6_masks)
+  done
+
+lemma lookup_pt_slot_authorised3:
+  "\<lbrace>\<exists>\<rhd> pd and K (is_subject aag pd) and
+    K (is_aligned pd 14 \<and> is_aligned vptr 16 \<and> vptr < kernel_base) and
+    valid_vspace_objs and valid_arch_state and equal_kernel_mappings and
+    valid_global_objs and pspace_aligned and pas_refined aag\<rbrace>
+   lookup_pt_slot pd vptr
+   \<lbrace>\<lambda>rv _.  \<forall>x\<in>set [rv, rv + 4 .e. rv + 0x3C]. is_subject aag (x && ~~ mask pt_bits)\<rbrace>, -"
+  apply (rule_tac Q'="\<lambda>rv s. is_aligned rv 6 \<and> (\<forall>x\<in>set [0, 4 .e. 0x3C].
+                                                  is_subject aag (x + rv && ~~ mask pt_bits))"
+               in hoare_post_imp_R)
+  apply (rule hoare_pre)
+  apply (wp lookup_pt_slot_is_aligned_6 lookup_pt_slot_authorised2)
+   apply (fastforce simp: vmsz_aligned_def pd_bits_def pageBits_def)
+  apply simp
+  apply (simp add: p_0x3C_shift)
+  done
+
+crunch respects[wp]: flush_page "integrity aag X st"
+  (simp: invalidateLocalTLB_VAASID_def ignore: do_machine_op)
+
+lemma find_pd_for_asid_pd_owned[wp]:
+  "\<lbrace>pas_refined aag and K (is_subject_asid aag asid)\<rbrace>
+   find_pd_for_asid asid
+   \<lbrace>\<lambda>rv _. is_subject aag rv\<rbrace>,-"
+  apply (wp find_pd_for_asid_authority2)
+  apply (auto simp: aag_has_Control_iff_owns)
+  done
+
+lemmas store_pte_pas_refined_simple =
+  store_pte_pas_refined[where pte=InvalidPTE, simplified pte_ref_simps, simplified]
+
+crunch pas_refined[wp]: unmap_page "pas_refined aag"
+  (wp: crunch_wps store_pde_pas_refined_simple store_pte_pas_refined_simple simp: crunch_simps)
+
+lemma unmap_page_respects:
+  "\<lbrace>integrity aag X st and pspace_aligned and valid_vspace_objs
+                       and K (is_subject_asid aag asid) and pas_refined aag
+                       and K (vmsz_aligned vptr sz \<and> vptr < kernel_base)\<rbrace>
+   unmap_page sz asid vptr pptr
+   \<lbrace>\<lambda>_. integrity aag X st\<rbrace>"
+  apply (rule hoare_gen_asm)
+  apply (simp add: unmap_page_def swp_def cong: vmpage_size.case_cong)
+  apply (rule hoare_pre)
+   apply (wpsimp wp: store_pte_respects store_pde_respects lookup_pt_slot_authorised
+                     hoare_drop_imps[where Q="\<lambda>rv. integrity aag X st"]
+               simp: is_aligned_6_masks is_aligned_mask[symmetric] cleanByVA_PoU_def
+          | wp (once) hoare_drop_imps
+                      mapM_set''[where f="(\<lambda>a. store_pte a InvalidPTE)"
+                                   and I="\<lambda>x s. is_subject aag (x && ~~ mask pt_bits)"
+                                   and Q="integrity aag X st"]
+                      mapM_set''[where f="(\<lambda>a. store_pde a InvalidPDE)"
+                                   and I="\<lambda>x s. is_subject aag (x && ~~ mask pd_bits)"
+                                   and Q="integrity aag X st"]
+          | wp (once) hoare_drop_imps[where R="\<lambda>rv s. rv"])+
+  done
+
+(* FIXME: CLAG *)
+lemmas do_machine_op_bind =
+  submonad_bind [OF submonad_do_machine_op submonad_do_machine_op submonad_do_machine_op]
+
+lemmas do_flush_defs =
+  cleanCacheRange_RAM_def cleanCacheRange_PoC_def cleanCacheRange_PoU_def branchFlushRange_def
+  invalidateCacheRange_RAM_def invalidateCacheRange_I_def cleanInvalidateCacheRange_RAM_def
+
+lemma do_flush_respects[wp]:
+  "do_machine_op (do_flush typ start end pstart) \<lbrace>integrity aag X st\<rbrace>"
+  by (cases "typ"; wpsimp wp: dmo_no_mem_respects simp: do_flush_def cache_machine_op_defs do_flush_defs)
+
+lemma invalidate_tlb_by_asid_respects[wp]:
+  "invalidate_tlb_by_asid asid \<lbrace>integrity aag X st\<rbrace>"
+  unfolding invalidate_tlb_by_asid_def
+  by (wpsimp wp: dmo_no_mem_respects simp: invalidateLocalTLB_ASID_def)
+
+lemma invalidate_tlb_by_asid_pas_refined[wp]:
+  "invalidate_tlb_by_asid asid \<lbrace>pas_refined aag\<rbrace>"
+  by (wpsimp wp: dmo_no_mem_respects simp: invalidate_tlb_by_asid_def invalidateLocalTLB_ASID_def)
+
+lemma perform_page_invocation_respects:
+  "\<lbrace>integrity aag X st and pas_refined aag and K (authorised_page_inv aag pgi)
+                       and valid_page_inv pgi and valid_vspace_objs
+                       and pspace_aligned and is_subject aag  \<circ> cur_thread\<rbrace>
+   perform_page_invocation pgi
+   \<lbrace>\<lambda>_. integrity aag X st\<rbrace>"
+proof -
+  (* does not work as elim rule with clarsimp, which hammers Ball in concl. *)
+  have set_tl_subset_mp: "\<And>xs a. a \<in> set (tl xs) \<Longrightarrow> a \<in> set xs" by (case_tac xs; clarsimp)
+  have hd_valid_slots:
+    "\<And>a xs s. valid_slots (Inl (a, xs)) s \<Longrightarrow> hd xs \<in> set xs"
+    "\<And>a xs s. valid_slots (Inr (a, xs)) s \<Longrightarrow> hd xs \<in> set xs"
+    by (simp_all add: valid_slots_def)
+  show ?thesis
+  apply (simp add: perform_page_invocation_def mapM_discarded swp_def
+                   valid_page_inv_def valid_unmap_def
+                   authorised_page_inv_def authorised_slots_def
+            split: page_invocation.split sum.split
+                   arch_cap.split option.split,
+         safe)
+        apply (wp set_cap_integrity_autarch unmap_page_respects
+                  mapM_x_and_const_wp[OF store_pte_respects] store_pte_respects
+                  mapM_x_and_const_wp[OF store_pde_respects] store_pde_respects
+               | elim conjE hd_valid_slots[THEN bspec[rotated]]
+               | clarsimp dest!: set_tl_subset_mp
+               | wpc )+
+   apply (clarsimp simp: cte_wp_at_caps_of_state cap_rights_update_def
+                         acap_rights_update_def update_map_data_def is_pg_cap_def
+                         valid_page_inv_def valid_cap_simps
+                  dest!: cap_master_cap_eqDs)
+   apply (drule (1) clas_caps_of_state)
+   apply (simp add: cap_links_asid_slot_def label_owns_asid_slot_def)
+   apply (auto dest: pas_refined_Control)[1]
+     apply (wpsimp wp: set_mrs_integrity_autarch set_message_info_integrity_autarch
+                 simp: ipc_buffer_has_auth_def)+
+  done
+qed
+
+(* FIXME MOVE *)
+crunch cdt[wp]: unmap_page "\<lambda>s. P (cdt s)"
+  (simp: crunch_simps wp: crunch_wps)
+
+lemma perform_page_invocation_pas_refined [wp]:
+  "\<lbrace>pas_refined aag and K (authorised_page_inv aag pgi) and valid_page_inv pgi\<rbrace>
+   perform_page_invocation pgi
+   \<lbrace>\<lambda>_. pas_refined aag\<rbrace>"
+  apply (simp add: perform_page_invocation_def mapM_discarded valid_page_inv_def valid_unmap_def
+                   swp_def authorised_page_inv_def authorised_slots_def
+             cong: page_invocation.case_cong sum.case_cong)
+  apply (rule hoare_pre)
+   apply wpc
+      apply (wp set_cap_pas_refined unmap_page_pas_refined case_sum_wp case_prod_wp get_cap_wp
+                mapM_x_and_const_wp[OF store_pte_pas_refined] hoare_vcg_all_lift
+                mapM_x_and_const_wp[OF store_pde_pas_refined] hoare_vcg_const_imp_lift
+             | (wp hoare_vcg_imp_lift, unfold disj_not1)
+             | strengthen clas_update_map_data_strg
+             | wpc | wps | simp)+
+  apply (case_tac pgi)
+      apply ((force simp: valid_slots_def pte_ref_def cte_wp_at_caps_of_state
+                          is_transferable_is_arch_update[symmetric]
+                          pde_ref2_def auth_graph_map_mem pas_refined_refl
+                   split: sum.splits)+)[2]
+    apply (clarsimp simp: cte_wp_at_caps_of_state is_transferable_is_arch_update[symmetric]
+                          pte_ref_def pde_ref2_def is_cap_simps is_pg_cap_def)
+    apply (frule(1) cap_cur_auth_caps_of_state, simp)
+    apply (intro impI conjI;
+           clarsimp; (* NB: for speed *)
+           clarsimp simp: update_map_data_def clas_no_asid aag_cap_auth_def
+                          cap_auth_conferred_def arch_cap_auth_conferred_def
+                          vspace_cap_rights_to_auth_def cli_no_irqs is_pg_cap_def
+                          pte_ref_def[simplified aag_cap_auth_def])+
+  done
+
+definition authorised_asid_control_inv :: "'a PAS \<Rightarrow> asid_control_invocation \<Rightarrow> bool" where
+ "authorised_asid_control_inv aag aci \<equiv>
+  case aci of MakePool frame slot parent base \<Rightarrow>
+    is_subject aag (fst slot) \<and> is_aligned frame pageBits \<and>
+    (\<forall>asid. is_subject_asid aag asid) \<and> is_subject aag (fst parent) \<and>
+            (\<forall>x \<in> {frame..frame + 2 ^ pageBits - 1}. is_subject aag x)"
+
+
+lemma integrity_arm_asid_table_entry_update':
+  "\<lbrakk> integrity aag X st s; atable = arm_asid_table (arch_state s);
+     (\<forall>asid'. asid' \<noteq> 0 \<and> asid_high_bits_of asid' = asid_high_bits_of asid
+             \<longrightarrow> is_subject_asid aag asid') \<rbrakk>
+     \<Longrightarrow> integrity aag X st (s\<lparr>arch_state := arch_state s\<lparr>arm_asid_table :=
+                                                          \<lambda>a. if a = asid_high_bits_of asid
+                                                              then v
+                                                              else atable a\<rparr>\<rparr>)"
+  by (clarsimp simp: integrity_def)
+
+lemma arm_asid_table_entry_update_integrity[wp]:
+ "\<lbrace>integrity aag X st and (\<lambda> s. atable = arm_asid_table (arch_state s)) and
+   K (\<forall>asid'. asid' \<noteq> 0 \<and> asid_high_bits_of asid' = asid_high_bits_of asid
+              \<longrightarrow> is_subject_asid aag asid')\<rbrace>
+  modify (\<lambda>s. s\<lparr>arch_state := arch_state s\<lparr>arm_asid_table := atable(asid_high_bits_of asid := v)\<rparr>\<rparr>)
+  \<lbrace>\<lambda>_. integrity aag X st\<rbrace>"
+  apply (wp | simp)+
+  apply (blast intro: integrity_arm_asid_table_entry_update')
+  done
+
+lemma perform_asid_control_invocation_respects:
+  "\<lbrace>integrity aag X st and K (authorised_asid_control_inv aag aci)\<rbrace>
+   perform_asid_control_invocation aci
+   \<lbrace>\<lambda>_. integrity aag X st\<rbrace>"
+  apply (simp add: perform_asid_control_invocation_def)
+  apply (rule hoare_pre)
+   apply (wpc, simp)
+   apply (wpsimp wp: set_cap_integrity_autarch cap_insert_integrity_autarch
+                     retype_region_integrity[where sz=12] static_imp_wp)
+  apply (clarsimp simp: authorised_asid_control_inv_def
+                        ptr_range_def page_bits_def add.commute
+                        range_cover_def obj_bits_api_def default_arch_object_def
+                        pageBits_def word_bits_def)
+  apply (subst is_aligned_neg_mask_eq[THEN sym], assumption)
+  apply (simp add: and_mask_eq_iff_shiftr_0 mask_zero)
+  done
+
+lemma pas_refined_set_asid_strg:
+  "pas_refined aag s \<and> is_subject aag pool \<and>
+   (\<forall>asid. asid_high_bits_of asid = base \<longrightarrow> is_subject_asid aag asid)
+   \<longrightarrow> pas_refined aag (s\<lparr>arch_state :=
+                          arch_state s\<lparr>arm_asid_table := (arm_asid_table (arch_state s))(base \<mapsto> pool)\<rparr>\<rparr>)"
+  apply (clarsimp simp: pas_refined_def state_objs_to_policy_def)
+  apply (erule state_asids_to_policy_aux.cases, simp_all split: if_split_asm)
+      apply (auto intro: state_asids_to_policy_aux.intros auth_graph_map_memI[OF sbta_vref]
+                 intro!: pas_refined_refl[simplified pas_refined_def state_objs_to_policy_def])
+  done
+
+lemma perform_asid_control_invocation_pas_refined [wp]:
+  "\<lbrace>pas_refined aag and pas_cur_domain aag and invs and valid_aci aci and ct_active
+                    and K (authorised_asid_control_inv aag aci)\<rbrace>
+   perform_asid_control_invocation aci
+   \<lbrace>\<lambda>_. pas_refined aag\<rbrace>"
+  apply (simp add: perform_asid_control_invocation_def)
+  apply (rule hoare_pre)
+   apply (wp cap_insert_pas_refined' static_imp_wp
+          | strengthen pas_refined_set_asid_strg
+          | wpc
+          | simp add: delete_objects_def2 fun_upd_def[symmetric])+
+      apply (wp retype_region_pas_refined'[where sz=pageBits]
+                hoare_vcg_ex_lift hoare_vcg_all_lift static_imp_wp hoare_wp_combs hoare_drop_imp
+                retype_region_invs_extras(4)[where sz = pageBits]
+             | simp add: do_machine_op_def split_def cte_wp_at_neg2)+
+      apply (wp retype_region_cte_at_other'[where sz=pageBits]
+                max_index_upd_invs_simple max_index_upd_caps_overlap_reserved
+                hoare_vcg_ex_lift set_cap_cte_wp_at hoare_vcg_disj_lift set_free_index_valid_pspace
+                set_cap_descendants_range_in set_cap_no_overlap get_cap_wp set_cap_caps_no_overlap
+                hoare_vcg_all_lift static_imp_wp retype_region_invs_extras
+                set_cap_pas_refined_not_transferable
+             | simp add: do_machine_op_def split_def cte_wp_at_neg2 region_in_kernel_window_def)+
+   apply (rename_tac frame slot parent base cap)
+   apply (case_tac slot, rename_tac slot_ptr slot_idx)
+   apply (case_tac parent, rename_tac parent_ptr parent_idx)
+   apply (rule_tac Q="\<lambda>rv s.
+             (\<exists>idx. cte_wp_at ((=) (UntypedCap False frame pageBits idx)) parent s) \<and>
+             (\<forall>x\<in>ptr_range frame pageBits. is_subject aag x) \<and>
+             pas_refined aag s \<and>
+             pas_cur_domain aag s \<and>
+             pspace_no_overlap_range_cover frame pageBits s \<and>
+             invs s \<and>
+             descendants_range_in
+               {frame..(frame && ~~ mask pageBits) + 2 ^ pageBits - 1} parent s \<and>
+             range_cover frame pageBits
+               (obj_bits_api (ArchObject ASIDPoolObj) 0) (Suc 0) \<and>
+             is_subject aag slot_ptr \<and>
+             is_subject aag parent_ptr \<and>
+             pas_cap_cur_auth aag (ArchObjectCap (ASIDPoolCap frame base)) \<and>
+             is_subject aag frame \<and>
+             (\<forall>x. asid_high_bits_of x = asid_high_bits_of base \<longrightarrow>
+                 is_subject_asid aag x)"
+             in hoare_strengthen_post)
+    apply (simp add: page_bits_def)
+    apply (wp add: delete_objects_pspace_no_overlap hoare_vcg_ex_lift
+                   delete_objects_descendants_range_in delete_objects_invs_ex
+                   delete_objects_pas_refined
+              del: Untyped_AI.delete_objects_pspace_no_overlap
+           | simp add: page_bits_def)+
+   apply clarsimp
+   apply (rename_tac s idx)
+   apply (frule untyped_cap_aligned, simp add: invs_valid_objs)
+   apply (clarsimp simp: cte_wp_at_def aag_cap_auth_def ptr_range_def pas_refined_refl
+                         cap_links_asid_slot_def cap_links_irq_def
+                         obj_bits_api_def default_arch_object_def retype_addrs_def)
+   apply (rule conjI, force intro: descendants_range_caps_no_overlapI
+                             simp: cte_wp_at_def)
+   apply (rule conjI)
+    apply (cut_tac s=s and ptr="(parent_ptr, parent_idx)" in cap_refs_in_kernel_windowD)
+      apply ((fastforce simp add: caps_of_state_def cap_range_def)+)[3]
+   apply (rule conjI, force simp: field_simps)
+   apply (rule conjI, fastforce)
+   apply (fastforce dest: caps_of_state_valid
+                    simp: caps_of_state_def free_index_of_def max_free_index_def valid_cap_def)
+  apply (clarsimp simp: valid_aci_def authorised_asid_control_inv_def)
+  apply (rename_tac frame slot_ptr slot_idx parent_ptr parent_idx base)
+  apply (subgoal_tac "is_aligned frame pageBits")
+   apply (clarsimp simp: cte_wp_at_caps_of_state)
+   apply (rule conjI)
+    apply (drule untyped_slots_not_in_untyped_range)
+         apply (erule empty_descendants_range_in)
+        apply (simp add: cte_wp_at_caps_of_state)
+       apply simp
+      apply (rule refl)
+     apply (rule subset_refl)
+    apply (simp add: page_bits_def)
+   apply (clarsimp simp: ptr_range_def invs_psp_aligned invs_valid_objs
+                         descendants_range_def2 empty_descendants_range_in page_bits_def)
+   apply ((strengthen refl | simp)+)?
+   apply (rule conjI, fastforce)
+   apply (rule conjI, fastforce intro: empty_descendants_range_in)
+   apply (rule conjI)
+    apply (clarsimp simp: range_cover_def obj_bits_api_def default_arch_object_def)
+    apply (subst is_aligned_neg_mask_eq[THEN sym], assumption)
+    apply (simp add: and_mask_eq_iff_shiftr_0 pageBits_def mask_zero)
+   apply (clarsimp simp: aag_cap_auth_def pas_refined_refl)
+   apply (drule_tac x=frame in bspec)
+    apply (simp add: is_aligned_no_overflow)
+   apply (clarsimp simp: pas_refined_refl cap_links_asid_slot_def
+                         label_owns_asid_slot_def cap_links_irq_def)
+  apply (fastforce dest: cte_wp_at_valid_objs_valid_cap simp: valid_cap_def cap_aligned_def)
+  done
+
+definition authorised_asid_pool_inv :: "'a PAS \<Rightarrow> asid_pool_invocation \<Rightarrow> bool" where
+ "authorised_asid_pool_inv aag api \<equiv>
+  case api of Assign asid pool_ptr ct_slot \<Rightarrow>
+    is_subject aag pool_ptr \<and> is_subject aag (fst ct_slot) \<and> asid \<noteq> 0 \<and>
+    (\<forall>asid'. asid_high_bits_of asid' = asid_high_bits_of asid \<and> asid' \<noteq> 0
+             \<longrightarrow> is_subject_asid aag asid')"
+
+lemma perform_asid_pool_invocation_respects:
+  "\<lbrace>integrity aag X st and K (authorised_asid_pool_inv aag api)\<rbrace>
+   perform_asid_pool_invocation api
+   \<lbrace>\<lambda>_. integrity aag X st\<rbrace>"
+  apply (simp add: perform_asid_pool_invocation_def)
+  apply (wpsimp wp: set_asid_pool_integrity_autarch get_cap_wp set_cap_integrity_autarch)
+  apply (auto iff: authorised_asid_pool_inv_def)
+  done
+
+lemma asid_pool_into_aag:
+  "\<lbrakk> kheap s p = Some (ArchObj (ASIDPool pool)); pool r = Some p'; pas_refined aag s \<rbrakk>
+     \<Longrightarrow> abs_has_auth_to aag Control p p'"
+  apply (rule pas_refined_mem [rotated], assumption)
+  apply (rule sta_vref)
+  apply (fastforce simp: state_vrefs_def vs_refs_no_global_pts_def intro!: graph_ofI)
+  done
+
+lemma asid_pool_uniqueness:
+  "\<lbrakk> ([VSRef (ucast (asid_high_bits_of asid)) None] \<rhd> p) s;
+     arm_asid_table (arch_state s) (asid_high_bits_of asid') = Some p;
+     invs s; \<forall>pt. \<not> ko_at (ArchObj (PageTable pt)) p s \<rbrakk>
+     \<Longrightarrow> asid_high_bits_of asid' = asid_high_bits_of asid"
+  apply (drule valid_vs_lookupD[OF vs_lookup_pages_vs_lookupI], clarsimp)
+  apply (drule vs_lookup_atI, drule valid_vs_lookupD[OF vs_lookup_pages_vs_lookupI], clarsimp)
+  apply (clarsimp dest!: obj_ref_elemD)
+  apply (drule(1) unique_table_refsD[where cps="caps_of_state s", rotated])
+    apply simp
+   apply (clarsimp simp: vs_cap_ref_def table_cap_ref_def up_ucast_inj_eq
+                  split: vmpage_size.splits option.splits cap.splits arch_cap.splits)+
+  done
+
+lemma perform_asid_pool_invocation_pas_refined [wp]:
+  "\<lbrace>pas_refined aag and invs and valid_apinv api and K (authorised_asid_pool_inv aag api)\<rbrace>
+   perform_asid_pool_invocation api
+   \<lbrace>\<lambda>_. pas_refined aag\<rbrace>"
+  apply (simp add: perform_asid_pool_invocation_def)
+  apply (rule hoare_pre)
+  apply (wp get_cap_auth_wp[where aag = aag] set_cap_pas_refined_not_transferable | wpc)+
+  apply (clarsimp simp: authorised_asid_pool_inv_def cap_links_asid_slot_def
+                        is_subject_asid_into_loas aag_cap_auth_def)
+  apply (clarsimp simp: cap_auth_conferred_def arch_cap_auth_conferred_def
+                        is_cap_simps is_page_cap_def auth_graph_map_mem
+                        pas_refined_all_auth_is_owns pas_refined_refl cli_no_irqs
+                        cte_wp_at_caps_of_state
+                 dest!: graph_ofD)
+  apply (clarsimp split: if_split_asm)
+   apply (clarsimp simp add: pas_refined_refl auth_graph_map_def2
+                             mask_asid_low_bits_ucast_ucast[symmetric]
+                             valid_apinv_def obj_at_def)
+   apply (drule(2) asid_pool_uniqueness)
+    apply (simp add: obj_at_def)
+   apply (case_tac "asid = 0"; simp add: pas_refined_refl)
+   apply (simp add: asid_low_high_bits[rotated, OF arg_cong[where f=ucast]])
+  apply (clarsimp simp: obj_at_def)
+  apply (frule (2) asid_pool_into_aag)
+  apply (drule kheap_eq_state_vrefsD)
+  apply (clarsimp simp: auth_graph_map_def2 pas_refined_refl)
+  apply (clarsimp simp: pas_refined_def vs_refs_no_global_pts_def)
+  apply (erule subsetD, erule state_asids_to_policy_aux.intros,
+         simp add: split_def, rule image_eqI[rotated], erule graph_ofI)
+  apply simp
+  done
+
+definition authorised_page_directory_inv :: "'a PAS \<Rightarrow> page_directory_invocation \<Rightarrow> bool" where
+  "authorised_page_directory_inv aag pdi \<equiv> True"
+
+definition authorised_arch_inv :: "'a PAS \<Rightarrow> arch_invocation \<Rightarrow> bool" where
+ "authorised_arch_inv aag ai \<equiv> case ai of
+     InvokePageTable pti \<Rightarrow> authorised_page_table_inv aag pti
+   | InvokePageDirectory pdi \<Rightarrow> authorised_page_directory_inv aag pdi
+   | InvokePage pgi \<Rightarrow> authorised_page_inv aag pgi
+   | InvokeASIDControl aci \<Rightarrow> authorised_asid_control_inv aag aci
+   | InvokeASIDPool api \<Rightarrow> authorised_asid_pool_inv aag api"
+
+crunch respects [wp]: perform_page_directory_invocation "integrity aag X st"
+  (ignore: do_machine_op)
+
+crunch pas_refined [wp]: perform_page_directory_invocation "pas_refined aag"
+
+lemma invoke_arch_respects:
+  "\<lbrace>integrity aag X st and K (authorised_arch_inv aag ai) and
+    pas_refined aag and invs and valid_arch_inv ai and is_subject aag \<circ> cur_thread\<rbrace>
+   arch_perform_invocation ai
+   \<lbrace>\<lambda>_. integrity aag X st\<rbrace>"
+  apply (simp add: arch_perform_invocation_def)
+  apply (wpsimp wp: perform_page_table_invocation_respects perform_page_invocation_respects
+                    perform_asid_control_invocation_respects perform_asid_pool_invocation_respects)
+  apply (auto simp: authorised_arch_inv_def valid_arch_inv_def)
+  done
+
+lemma invoke_arch_pas_refined:
+  "\<lbrace>pas_refined aag and pas_cur_domain aag and invs and ct_active
+                    and valid_arch_inv ai and K (authorised_arch_inv aag ai)\<rbrace>
+   arch_perform_invocation ai
+   \<lbrace>\<lambda>_. pas_refined aag\<rbrace>"
+  apply (simp add: arch_perform_invocation_def valid_arch_inv_def)
+  apply (rule hoare_pre)
+  apply (wp | wpc)+
+  apply (fastforce simp add: authorised_arch_inv_def)
+  done
+
+lemma create_mapping_entries_authorised_slots [wp]:
+  "\<lbrace>\<exists>\<rhd> pd and invs and pas_refined aag and
+    K (is_subject aag pd \<and> is_aligned pd pd_bits \<and>
+       vmsz_aligned vptr vmpage_size \<and> vptr < kernel_base \<and>
+       (\<forall>a\<in>vspace_cap_rights_to_auth rights.
+          \<forall>p\<in>ptr_range (ptrFromPAddr base) (pageBitsForSize vmpage_size). aag_has_auth_to aag a p))\<rbrace>
+   create_mapping_entries base vptr vmpage_size rights attrib pd
+   \<lbrace>\<lambda>rv _. authorised_slots aag rv\<rbrace>, -"
+  unfolding authorised_slots_def
+  apply (rule hoare_gen_asmE)
+  apply (cases vmpage_size)
+     apply (wp lookup_pt_slot_authorised | simp add: pte_ref_simps | fold validE_R_def)+
+     apply (auto simp: pd_bits_def pageBits_def)[1]
+    apply (wp lookup_pt_slot_authorised2
+           | simp add: pte_ref_simps largePagePTE_offsets_def
+           | fold validE_R_def)+
+    apply (auto simp: pd_bits_def pageBits_def vmsz_aligned_def)[1]
+   apply (wp | simp)+
+   apply (auto simp: pde_ref2_def lookup_pd_slot_pd)[1]
+  apply (wp | simp add: superSectionPDE_offsets_def)+
+  apply (auto simp: pde_ref2_def vmsz_aligned_def lookup_pd_slot_add_eq)
+  done
+
+lemma pageBitsForSize_le_t29:
+  "pageBitsForSize sz \<le> 29"
+  by (cases sz, simp_all)
+
+lemma x_t2n_sub_1_neg_mask:
+  "\<lbrakk> is_aligned x n; n \<le> m \<rbrakk>
+     \<Longrightarrow> x + 2 ^ n - 1 && ~~ mask m = x && ~~ mask m"
+  apply (erule is_aligned_get_word_bits)
+   apply (rule trans, rule mask_lower_twice[symmetric], assumption)
+   apply (subst add_diff_eq[symmetric], subst is_aligned_add_helper, assumption)
+    apply simp+
+  apply (simp add: mask_def power_overflow)
+  done
+
+lemmas vmsz_aligned_t2n_neg_mask =
+  x_t2n_sub_1_neg_mask[OF _ pageBitsForSize_le_t29, folded vmsz_aligned_def]
+
+lemma decode_arch_invocation_authorised:
+  "\<lbrace>invs and pas_refined aag and cte_wp_at ((=) (ArchObjectCap cap)) slot
+         and (\<lambda>s. \<forall>(cap, slot) \<in> set excaps. cte_wp_at ((=) cap) slot s)
+         and K (\<forall>(cap, slot) \<in> {(ArchObjectCap cap, slot)} \<union> set excaps.
+                  aag_cap_auth aag (pasObjectAbs aag (fst slot)) cap \<and>
+                  is_subject aag (fst slot) \<and>
+                  (\<forall>v \<in> cap_asid' cap. is_subject_asid aag v))\<rbrace>
+   arch_decode_invocation label msg x_slot slot cap excaps
+   \<lbrace>\<lambda>rv _. authorised_arch_inv aag rv\<rbrace>,-"
+  unfolding arch_decode_invocation_def authorised_arch_inv_def aag_cap_auth_def
+  apply (rule hoare_pre)
+   apply (simp add: split_def Let_def split del: if_split
+              cong: cap.case_cong arch_cap.case_cong if_cong option.case_cong)
+   apply (wp select_wp whenE_throwError_wp check_vp_wpR
+             find_pd_for_asid_authority2
+          | wpc
+          | simp add: authorised_asid_control_inv_def authorised_page_inv_def
+                      authorised_page_directory_inv_def
+                 del: hoare_True_E_R
+                 split del: if_split)+
+  apply (clarsimp simp: authorised_asid_pool_inv_def authorised_page_table_inv_def
+                        neq_Nil_conv invs_psp_aligned invs_vspace_objs cli_no_irqs)
+  apply (drule cte_wp_valid_cap, clarsimp+)
+  apply (cases cap; simp)
+      \<comment> \<open>asid pool\<close>
+     apply (find_goal \<open>match premises in "cap = ASIDPoolCap _ _" \<Rightarrow> succeed\<close>)
+     subgoal for s obj_ref asid
+       by (clarsimp simp: cap_auth_conferred_def arch_cap_auth_conferred_def is_page_cap_def
+                          pas_refined_all_auth_is_owns asid_high_bits_of_add_ucast valid_cap_simps)
+     \<comment> \<open>ControlCap\<close>
+    apply (find_goal \<open>match premises in "cap = ASIDControlCap" \<Rightarrow> succeed\<close>)
+    subgoal
+      apply (clarsimp simp: neq_Nil_conv split_def valid_cap_simps)
+      apply (cases excaps, solves simp)
+      apply (clarsimp simp: neq_Nil_conv aag_has_Control_iff_owns)
+      apply (drule cte_wp_at_valid_objs_valid_cap, clarsimp)
+      apply (clarsimp simp: valid_cap_def cap_aligned_def)
+      apply (clarsimp simp: is_cap_simps cap_auth_conferred_def
+                            pas_refined_all_auth_is_owns aag_cap_auth_def)
+      done
+   \<comment> \<open>PageCap\<close>
+   apply (find_goal \<open>match premises in "cap = PageCap _ _ _ _ _" \<Rightarrow> succeed\<close>)
+   subgoal for s is_dev obj_ref cap_rights vmpage_size mapping
+     apply (clarsimp simp: valid_cap_simps cli_no_irqs)
+     apply (cases "invocation_type label"; (solves \<open>simp\<close>)?)
+     apply (find_goal \<open>match premises in "_ = ArchInvocationLabel _" \<Rightarrow> succeed\<close>)
+     apply (rename_tac archlabel)
+     apply (case_tac archlabel; (solves \<open>simp\<close>)?)
+       \<comment> \<open>Map\<close>
+      apply (find_goal \<open>match premises in "_ = ARMPageMap" \<Rightarrow> succeed\<close>)
+      subgoal
+       apply (clarsimp simp: cap_auth_conferred_def arch_cap_auth_conferred_def is_cap_simps is_page_cap_def
+                             pas_refined_all_auth_is_owns)
+       apply (rule conjI)
+        apply (clarsimp simp: is_page_cap_def pas_refined_all_auth_is_owns
+                              aag_cap_auth_def cli_no_irqs cap_links_asid_slot_def)
+        apply (simp only: linorder_not_le kernel_base_less_observation
+                          vmsz_aligned_t2n_neg_mask simp_thms)
+         apply (clarsimp simp: cap_auth_conferred_def arch_cap_auth_conferred_def
+                               vspace_cap_rights_to_auth_def mask_vm_rights_def
+                               validate_vm_rights_def vm_read_only_def vm_kernel_only_def)
+        apply clarsimp
+        apply (clarsimp simp: cap_auth_conferred_def arch_cap_auth_conferred_def aag_cap_auth_def
+                               cli_no_irqs vspace_cap_rights_to_auth_def mask_vm_rights_def
+                              validate_vm_rights_def vm_read_only_def vm_kernel_only_def)
+       done
+     \<comment> \<open>Unmap\<close>
+     subgoal by (simp add: aag_cap_auth_def cli_no_irqs)
+     done
+  \<comment> \<open>PageTableCap\<close>
+  apply (find_goal \<open>match premises in "cap = PageTableCap _ _" \<Rightarrow> succeed\<close>)
+  subgoal for s word option
+    apply (cases "invocation_type label"; (solves \<open>simp\<close>)?)
+    apply (find_goal \<open>match premises in "_ = ArchInvocationLabel _" \<Rightarrow> succeed\<close>)
+    apply (rename_tac archlabel)
+    apply (case_tac archlabel; (solves \<open>simp\<close>)?)
+     \<comment> \<open>PTMap\<close>
+     apply (find_goal \<open>match premises in "_ = ARMPageTableMap" \<Rightarrow> succeed\<close>)
+     apply (clarsimp simp: aag_cap_auth_def cli_no_irqs cap_links_asid_slot_def
+                           cap_auth_conferred_def arch_cap_auth_conferred_def is_page_cap_def
+                           pde_ref2_def pas_refined_all_auth_is_owns pas_refined_refl
+                           pd_shifting[folded pd_bits_14])
+    \<comment> \<open>Unmap\<close>
+    apply (find_goal \<open>match premises in "_ = ARMPageTableUnmap" \<Rightarrow> succeed\<close>)
+    subgoal
+      apply (clarsimp simp: aag_cap_auth_def cli_no_irqs cap_links_asid_slot_def
+                            cap_auth_conferred_def arch_cap_auth_conferred_def is_page_cap_def
+                            pde_ref2_def pas_refined_all_auth_is_owns pas_refined_refl)
+      apply (subgoal_tac "x && ~~ mask pt_bits = word")
+       apply simp
+      apply (clarsimp simp: valid_cap_simps cap_aligned_def split: if_split_asm)
+      apply (subst (asm) upto_enum_step_subtract)
+      apply (subgoal_tac "is_aligned word pt_bits")
+       apply (simp add: is_aligned_no_overflow)
+      apply (simp add: pt_bits_def pageBits_def)
+      apply simp
+      apply (subst (asm) upto_enum_step_red [where us = 2, simplified])
+      apply (simp add: pt_bits_def pageBits_def word_bits_conv)
+      apply (simp add: pt_bits_def pageBits_def word_bits_conv)
+      apply clarsimp
+      apply (subst is_aligned_add_helper)
+      apply (simp add: pt_bits_def pageBits_def)
+      apply (erule word_less_power_trans_ofnat [where k = 2, simplified])
+        apply (simp add: pt_bits_def pageBits_def)
+       apply (simp add: pt_bits_def pageBits_def word_bits_conv)
+      apply simp
+      done
+    done
+  done
+
+crunch pas_refined[wp]: invalidate_asid_entry "pas_refined aag"
+  (wp: crunch_wps simp: crunch_simps)
+
+crunch pas_refined[wp]: flush_space "pas_refined aag"
+  (wp: crunch_wps simp: crunch_simps)
+
+lemma delete_asid_pas_refined[wp]:
+  "delete_asid asid pd \<lbrace>pas_refined aag\<rbrace>"
+  apply (simp add: delete_asid_def)
+  apply (wp | wpc)+
+  apply (clarsimp simp add: split_def Ball_def obj_at_def)
+  apply (rule conjI)
+   apply (clarsimp dest!: auth_graph_map_memD graph_ofD)
+   apply (erule pas_refined_mem[OF sta_vref, rotated])
+   apply (fastforce simp: state_vrefs_def vs_refs_no_global_pts_def
+                         image_def graph_of_def split: if_split_asm)
+  apply (clarsimp simp: pas_refined_def dest!: graph_ofD)
+  apply (erule subsetD, erule state_asids_to_policy_aux.intros)
+  apply (fastforce simp: state_vrefs_def vs_refs_no_global_pts_def
+                        graph_of_def image_def split: if_split_asm)
+  done
+
+lemma delete_asid_pool_pas_refined [wp]:
+  "delete_asid_pool param_a param_b \<lbrace>pas_refined aag\<rbrace>"
+  unfolding delete_asid_pool_def
+  apply (wp | wpc | simp)+
+      apply (rule_tac Q = "\<lambda>_ s. pas_refined aag s \<and>
+                                 asid_table = arm_asid_table (arch_state s)" in hoare_post_imp)
+       apply clarsimp
+       apply (erule pas_refined_clear_asid)
+      apply (wp mapM_wp' | simp)+
+  done
+
+crunch respects[wp]: invalidate_asid_entry "integrity aag X st"
+
+crunch respects[wp]: flush_space "integrity aag X st"
+  (ignore: do_machine_op simp: invalidateLocalTLB_ASID_def cleanCaches_PoU_def
+           dsb_def clean_D_PoU_def invalidate_I_PoU_def do_machine_op_bind)
+
+lemma delete_asid_pool_respects[wp]:
+  "\<lbrace>integrity aag X st and
+    K (\<forall>asid'. asid' \<noteq> 0 \<and> asid_high_bits_of asid' = asid_high_bits_of x
+               \<longrightarrow> is_subject_asid aag asid')\<rbrace>
+   delete_asid_pool x y
+   \<lbrace>\<lambda>_. integrity aag X st\<rbrace>"
+  unfolding delete_asid_pool_def
+  apply simp
+  apply (wp mapM_wp[OF _ subset_refl] | simp)+
+  done
+
+lemma set_asid_pool_respects_clear:
+  "\<lbrace>integrity aag X st and (\<lambda>s. \<forall>pool'. ko_at (ArchObj (arch_kernel_obj.ASIDPool pool')) ptr s
+                                        \<longrightarrow> asid_pool_integrity {pasSubject aag} aag pool' pool)\<rbrace>
+   set_asid_pool ptr pool
+   \<lbrace>\<lambda>_. integrity aag X st\<rbrace>"
+  apply (simp add: set_asid_pool_def)
+  apply (wpsimp wp: set_object_wp_strong
+              simp: obj_at_def a_type_def
+             split: Structures_A.kernel_object.split_asm arch_kernel_obj.split_asm if_splits)
+  apply (erule integrity_trans)
+  apply (clarsimp simp: integrity_def)
+  apply (rule tro_arch; fastforce simp: arch_integrity_obj_atomic.simps)
+  done
+
+lemma delete_asid_respects:
+  "\<lbrace>integrity aag X st and pas_refined aag and invs and K (is_subject aag pd)\<rbrace>
+   delete_asid asid pd
+   \<lbrace>\<lambda>_. integrity aag X st\<rbrace>"
+  by (wpsimp wp: set_asid_pool_respects_clear hoare_vcg_all_lift
+           simp: obj_at_def pas_refined_refl delete_asid_def asid_pool_integrity_def)
+
+end
+
+
+context begin interpretation Arch .
+
+requalify_facts
+  invoke_arch_pas_refined
+  invoke_arch_respects
+  decode_arch_invocation_authorised
+
+requalify_consts
+  authorised_arch_inv
+
+end
+
+end
